Make rename module include mutual inductive type

examples/tests/RenameMe.hs
@@ -1,3 +1,7 @@
 module RenameMe where
 
+import RenameMeToo
+
+data Odd = One | Even Even
+
 x = True
