examples/ghc/lib/IdInfo.v
@@ -1,1 +1,332 @@
-../manual/IdInfo.v
+(* Default settings (from HsToCoq.Coq.Preamble) *)
+
+Generalizable All Variables.
+
+Unset Implicit Arguments.
+Set Maximal Implicit Insertion.
+Unset Strict Implicit.
+Unset Printing Implicit Defensive.
+
+Require Coq.Program.Tactics.
+Require Coq.Program.Wf.
+
+(* Preamble *)
+
+Require GHC.Err.
+Require GHC.Base.
+
+(* We might put these elsewhere, but these are some types that we 
+   can use for untying the knots in DataCon/Class/PatSyn *)
+
+Parameter DataConId : Type.
+Parameter ClassId   : Type.
+Parameter PatSynId  : Type.
+
+Parameter Default_DataConId : GHC.Err.Default DataConId.
+Parameter Default_ClassId   : GHC.Err.Default ClassId.
+Parameter Default_PatSynId  : GHC.Err.Default PatSynId.
+
+Parameter Eq_PatSynId  : Base.Eq_ PatSynId.
+Parameter Eq_ClassId   : Base.Eq_ ClassId.
+Parameter Eq_DataConId : Base.Eq_ DataConId.
+
+Parameter Ord_PatSynId  : Base.Ord PatSynId.
+Parameter Ord_ClassId   : Base.Ord ClassId.
+Parameter Ord_DataConId : Base.Ord DataConId.
+
+
+(*
+-- An 'IdInfo' gives /optional/ information about an 'Id'.  If
+-- present it never lies, but it may not be present, in which case there
+-- is always a conservative assumption which can be made.
+
+-- Most of the 'IdInfo' gives information about the value, or definition, of
+-- the 'Id', independent of its usage. Exceptions to this
+-- are 'demandInfo', 'occInfo', 'oneShotInfo' and 'callArityInfo'.
+--
+
+data IdInfo
+  = IdInfo {
+        arityInfo       :: !ArityInfo,          -- ^ 'Id' arity
+        ruleInfo        :: RuleInfo,            -- ^ Specialisations of the 'Id's function which exist
+                                                -- See Note [Specialisations and RULES in IdInfo]
+        unfoldingInfo   :: Unfolding,           -- ^ The 'Id's unfolding
+        cafInfo         :: CafInfo,             -- ^ 'Id' CAF info
+        oneShotInfo     :: OneShotInfo,         -- ^ Info about a lambda-bound variable, if the 'Id' is one
+        inlinePragInfo  :: InlinePragma,        -- ^ Any inline pragma atached to the 'Id'
+        occInfo         :: OccInfo,             -- ^ How the 'Id' occurs in the program
+
+        strictnessInfo  :: StrictSig,      --  ^ A strictness signature
+
+        demandInfo      :: Demand,       -- ^ ID demand information
+        callArityInfo   :: !ArityInfo,   -- ^ How this is called.
+                                         -- n <=> all calls have at least n arguments
+
+        levityInfo      :: LevityInfo    -- ^ when applied, will this Id ever have a levity-polymorphic type?
+    }
+
+*)
+
+Parameter IdInfo        : Type.
+Parameter vanillaIdInfo : IdInfo.
+Parameter noCafIdInfo   : IdInfo.
+
+Instance Default_IdInfo : GHC.Err.Default IdInfo :=
+  GHC.Err.Build_Default _ vanillaIdInfo.
+
+(* -------------------- *)
+
+Parameter RuleInfo : Type.
+Parameter emptyRuleInfo : RuleInfo.
+Parameter isEmptyRuleInfo : RuleInfo -> bool.
+
+Instance Default_RuleInfo : GHC.Err.Default RuleInfo :=
+  GHC.Err.Build_Default _ emptyRuleInfo.
+
+
+(* -------------------- *)
+
+(*
+Parameter RecSelParent : Type.
+Parameter Default_RecSelParent : GHC.Err.Default RecSelParent.
+
+Parameter Eq___RecSelParent : GHC.Base.Eq_ RecSelParent.
+*)
+
+(* Converted imports: *)
+
+Require BasicTypes.
+Require GHC.Base.
+Require GHC.Err.
+Require GHC.Num.
+Require Module.
+Import GHC.Base.Notations.
+Import GHC.Num.Notations.
+
+(* Converted type declarations: *)
+
+Definition TickBoxId :=
+  GHC.Num.Int%type.
+
+Inductive TickBoxOp : Type := TickBox : Module.Module -> TickBoxId -> TickBoxOp.
+
+Inductive RecSelParent : Type
+  := RecSelData : unit -> RecSelParent
+  |  RecSelPatSyn : PatSynId -> RecSelParent.
+
+Inductive LevityInfo : Type
+  := NoLevityInfo : LevityInfo
+  |  NeverLevityPolymorphic : LevityInfo.
+
+Definition InlinePragInfo :=
+  BasicTypes.InlinePragma%type.
+
+Inductive IdDetails : Type
+  := VanillaId : IdDetails
+  |  RecSelId : RecSelParent -> bool -> IdDetails
+  |  DataConWorkId : DataConId -> IdDetails
+  |  DataConWrapId : DataConId -> IdDetails
+  |  ClassOpId : ClassId -> IdDetails
+  |  PrimOpId : unit -> IdDetails
+  |  FCallId : unit -> IdDetails
+  |  TickBoxOpId : TickBoxOp -> IdDetails
+  |  DFunId : bool -> IdDetails
+  |  CoVarId : IdDetails
+  |  JoinId : BasicTypes.JoinArity -> IdDetails.
+
+Inductive CafInfo : Type := MayHaveCafRefs : CafInfo |  NoCafRefs : CafInfo.
+
+Definition ArityInfo :=
+  BasicTypes.Arity%type.
+
+Instance Default__LevityInfo : GHC.Err.Default LevityInfo :=
+  GHC.Err.Build_Default _ NoLevityInfo.
+
+Instance Default__IdDetails : GHC.Err.Default IdDetails :=
+  GHC.Err.Build_Default _ VanillaId.
+
+Instance Default__CafInfo : GHC.Err.Default CafInfo :=
+  GHC.Err.Build_Default _ MayHaveCafRefs.
+
+Definition sel_naughty (arg_0__ : IdDetails) :=
+  match arg_0__ with
+  | VanillaId =>
+      GHC.Err.error (GHC.Base.hs_string__
+                     "Partial record selector: field `sel_naughty' has no match in constructor `VanillaId' of type `IdDetails'")
+  | RecSelId _ sel_naughty => sel_naughty
+  | DataConWorkId _ =>
+      GHC.Err.error (GHC.Base.hs_string__
+                     "Partial record selector: field `sel_naughty' has no match in constructor `DataConWorkId' of type `IdDetails'")
+  | DataConWrapId _ =>
+      GHC.Err.error (GHC.Base.hs_string__
+                     "Partial record selector: field `sel_naughty' has no match in constructor `DataConWrapId' of type `IdDetails'")
+  | ClassOpId _ =>
+      GHC.Err.error (GHC.Base.hs_string__
+                     "Partial record selector: field `sel_naughty' has no match in constructor `ClassOpId' of type `IdDetails'")
+  | PrimOpId _ =>
+      GHC.Err.error (GHC.Base.hs_string__
+                     "Partial record selector: field `sel_naughty' has no match in constructor `PrimOpId' of type `IdDetails'")
+  | FCallId _ =>
+      GHC.Err.error (GHC.Base.hs_string__
+                     "Partial record selector: field `sel_naughty' has no match in constructor `FCallId' of type `IdDetails'")
+  | TickBoxOpId _ =>
+      GHC.Err.error (GHC.Base.hs_string__
+                     "Partial record selector: field `sel_naughty' has no match in constructor `TickBoxOpId' of type `IdDetails'")
+  | DFunId _ =>
+      GHC.Err.error (GHC.Base.hs_string__
+                     "Partial record selector: field `sel_naughty' has no match in constructor `DFunId' of type `IdDetails'")
+  | CoVarId =>
+      GHC.Err.error (GHC.Base.hs_string__
+                     "Partial record selector: field `sel_naughty' has no match in constructor `CoVarId' of type `IdDetails'")
+  | JoinId _ =>
+      GHC.Err.error (GHC.Base.hs_string__
+                     "Partial record selector: field `sel_naughty' has no match in constructor `JoinId' of type `IdDetails'")
+  end.
+(* Midamble *)
+
+Require GHC.Err.
+
+
+Instance Default_TickBoxOp : GHC.Err.Default TickBoxOp :=
+  GHC.Err.Build_Default _ (TickBox GHC.Err.default GHC.Err.default).
+
+Instance Default_CafInfo : GHC.Err.Default CafInfo :=
+  GHC.Err.Build_Default _ MayHaveCafRefs.
+
+(*
+Instance Default_IdInfo : GHC.Err.Default IdInfo :=
+  GHC.Err.Build_Default _ (Mk_IdInfo GHC.Err.default GHC.Err.default GHC.Err.default
+                         GHC.Err.default GHC.Err.default GHC.Err.default GHC.Err.default
+                         GHC.Err.default GHC.Err.default GHC.Err.default).
+*)
+(* Converted value declarations: *)
+
+(* Translating `instance Outputable__LevityInfo' failed: OOPS! Cannot find
+   information for class Qualified "Outputable" "Outputable" unsupported *)
+
+(* Translating `instance Outputable__IdDetails' failed: OOPS! Cannot find
+   information for class Qualified "Outputable" "Outputable" unsupported *)
+
+(* Translating `instance Outputable__TickBoxOp' failed: OOPS! Cannot find
+   information for class Qualified "Outputable" "Outputable" unsupported *)
+
+(* Translating `instance Outputable__CafInfo' failed: OOPS! Cannot find
+   information for class Qualified "Outputable" "Outputable" unsupported *)
+
+(* Translating `instance Outputable__RecSelParent' failed: OOPS! Cannot find
+   information for class Qualified "Outputable" "Outputable" unsupported *)
+
+Local Definition Eq___LevityInfo_op_zeze__ : LevityInfo -> LevityInfo -> bool :=
+  fun arg_0__ arg_1__ =>
+    match arg_0__, arg_1__ with
+    | NoLevityInfo, NoLevityInfo => true
+    | NeverLevityPolymorphic, NeverLevityPolymorphic => true
+    | _, _ => false
+    end.
+
+Local Definition Eq___LevityInfo_op_zsze__ : LevityInfo -> LevityInfo -> bool :=
+  fun x y => negb (Eq___LevityInfo_op_zeze__ x y).
+
+Program Instance Eq___LevityInfo : GHC.Base.Eq_ LevityInfo :=
+  fun _ k =>
+    k {| GHC.Base.op_zeze____ := Eq___LevityInfo_op_zeze__ ;
+         GHC.Base.op_zsze____ := Eq___LevityInfo_op_zsze__ |}.
+
+Local Definition Ord__CafInfo_compare : CafInfo -> CafInfo -> comparison :=
+  fun a b =>
+    match a with
+    | MayHaveCafRefs => match b with | MayHaveCafRefs => Eq | _ => Lt end
+    | NoCafRefs => match b with | NoCafRefs => Eq | _ => Gt end
+    end.
+
+Local Definition Ord__CafInfo_op_zl__ : CafInfo -> CafInfo -> bool :=
+  fun a b =>
+    match a with
+    | MayHaveCafRefs => match b with | MayHaveCafRefs => false | _ => true end
+    | NoCafRefs => match b with | NoCafRefs => false | _ => false end
+    end.
+
+Local Definition Ord__CafInfo_op_zlze__ : CafInfo -> CafInfo -> bool :=
+  fun a b => negb (Ord__CafInfo_op_zl__ b a).
+
+Local Definition Ord__CafInfo_min : CafInfo -> CafInfo -> CafInfo :=
+  fun x y => if Ord__CafInfo_op_zlze__ x y : bool then x else y.
+
+Local Definition Ord__CafInfo_max : CafInfo -> CafInfo -> CafInfo :=
+  fun x y => if Ord__CafInfo_op_zlze__ x y : bool then y else x.
+
+Local Definition Ord__CafInfo_op_zgze__ : CafInfo -> CafInfo -> bool :=
+  fun a b => negb (Ord__CafInfo_op_zl__ a b).
+
+Local Definition Ord__CafInfo_op_zg__ : CafInfo -> CafInfo -> bool :=
+  fun a b => Ord__CafInfo_op_zl__ b a.
+
+Local Definition Eq___CafInfo_op_zeze__ : CafInfo -> CafInfo -> bool :=
+  fun arg_0__ arg_1__ =>
+    match arg_0__, arg_1__ with
+    | MayHaveCafRefs, MayHaveCafRefs => true
+    | NoCafRefs, NoCafRefs => true
+    | _, _ => false
+    end.
+
+Local Definition Eq___CafInfo_op_zsze__ : CafInfo -> CafInfo -> bool :=
+  fun x y => negb (Eq___CafInfo_op_zeze__ x y).
+
+Program Instance Eq___CafInfo : GHC.Base.Eq_ CafInfo :=
+  fun _ k =>
+    k {| GHC.Base.op_zeze____ := Eq___CafInfo_op_zeze__ ;
+         GHC.Base.op_zsze____ := Eq___CafInfo_op_zsze__ |}.
+
+Program Instance Ord__CafInfo : GHC.Base.Ord CafInfo :=
+  fun _ k =>
+    k {| GHC.Base.op_zl____ := Ord__CafInfo_op_zl__ ;
+         GHC.Base.op_zlze____ := Ord__CafInfo_op_zlze__ ;
+         GHC.Base.op_zg____ := Ord__CafInfo_op_zg__ ;
+         GHC.Base.op_zgze____ := Ord__CafInfo_op_zgze__ ;
+         GHC.Base.compare__ := Ord__CafInfo_compare ;
+         GHC.Base.max__ := Ord__CafInfo_max ;
+         GHC.Base.min__ := Ord__CafInfo_min |}.
+
+Local Definition Eq___RecSelParent_op_zeze__
+   : RecSelParent -> RecSelParent -> bool :=
+  fun arg_0__ arg_1__ =>
+    match arg_0__, arg_1__ with
+    | RecSelData a1, RecSelData b1 => ((a1 GHC.Base.== b1))
+    | RecSelPatSyn a1, RecSelPatSyn b1 => ((a1 GHC.Base.== b1))
+    | _, _ => false
+    end.
+
+Local Definition Eq___RecSelParent_op_zsze__
+   : RecSelParent -> RecSelParent -> bool :=
+  fun x y => negb (Eq___RecSelParent_op_zeze__ x y).
+
+Program Instance Eq___RecSelParent : GHC.Base.Eq_ RecSelParent :=
+  fun _ k =>
+    k {| GHC.Base.op_zeze____ := Eq___RecSelParent_op_zeze__ ;
+         GHC.Base.op_zsze____ := Eq___RecSelParent_op_zsze__ |}.
+
+Definition coVarDetails : IdDetails :=
+  CoVarId.
+
+Definition isCoVarDetails : IdDetails -> bool :=
+  fun arg_0__ => match arg_0__ with | CoVarId => true | _ => false end.
+
+Definition isJoinIdDetails_maybe : IdDetails -> option BasicTypes.JoinArity :=
+  fun arg_0__ =>
+    match arg_0__ with
+    | JoinId join_arity => Some join_arity
+    | _ => None
+    end.
+
+Definition mayHaveCafRefs : CafInfo -> bool :=
+  fun arg_0__ => match arg_0__ with | MayHaveCafRefs => true | _ => false end.
+
+Definition unknownArity : BasicTypes.Arity :=
+  #0.
+
+(* External variables:
+     ClassId DataConId Eq Gt Lt None PatSynId Some bool comparison false negb option
+     true unit BasicTypes.Arity BasicTypes.InlinePragma BasicTypes.JoinArity
+     GHC.Base.Eq_ GHC.Base.Ord GHC.Base.op_zeze__ GHC.Err.Build_Default
+     GHC.Err.Default GHC.Err.error GHC.Num.Int GHC.Num.fromInteger Module.Module
+*)
