examples/ghc/lib/Util.v
@@ -1,1 +1,655 @@
-../manual/Util.v
+(* Default settings (from HsToCoq.Coq.Preamble) *)
+
+Generalizable All Variables.
+
+Unset Implicit Arguments.
+Set Maximal Implicit Insertion.
+Unset Strict Implicit.
+Unset Printing Implicit Defensive.
+
+Require Coq.Program.Tactics.
+Require Coq.Program.Wf.
+
+(* Converted imports: *)
+
+Require Coq.Init.Datatypes.
+Require Coq.Lists.List.
+Require Data.Bits.
+Require Data.Either.
+Require Data.Foldable.
+Require Data.OldList.
+Require GHC.Base.
+Require GHC.Char.
+Require GHC.DeferredFix.
+Require GHC.Err.
+Require GHC.List.
+Require GHC.Num.
+Require Panic.
+Import Data.Bits.Notations.
+Import GHC.Base.Notations.
+Import GHC.Num.Notations.
+
+(* Converted type declarations: *)
+
+Definition Suffix :=
+  GHC.Base.String%type.
+
+Inductive OverridingBool : Type
+  := Auto : OverridingBool
+  |  Always : OverridingBool
+  |  Never : OverridingBool.
+
+Definition HasDebugCallStack :=
+  unit.
+
+Inductive Direction : Type := Forwards : Direction |  Backwards : Direction.
+
+Instance Default__OverridingBool : GHC.Err.Default OverridingBool :=
+  GHC.Err.Build_Default _ Auto.
+
+Instance Default__Direction : GHC.Err.Default Direction :=
+  GHC.Err.Build_Default _ Forwards.
+(* Converted value declarations: *)
+
+(* Translating `instance Show__OverridingBool' failed: OOPS! Cannot find
+   information for class Qualified "GHC.Show" "Show" unsupported *)
+
+Definition all2 {a} {b} : (a -> b -> bool) -> list a -> list b -> bool :=
+  fix all2 arg_0__ arg_1__ arg_2__
+        := match arg_0__, arg_1__, arg_2__ with
+           | _, nil, nil => true
+           | p, cons x xs, cons y ys => andb (p x y) (all2 p xs ys)
+           | _, _, _ => false
+           end.
+
+Definition atLength {a} {b}
+   : (list a -> b) -> b -> list a -> GHC.Num.Int -> b :=
+  fun atLenPred atEnd ls0 n0 =>
+    let fix go arg_0__ arg_1__
+              := match arg_0__, arg_1__ with
+                 | num_2__, ls =>
+                     if num_2__ GHC.Base.== #0 : bool then atLenPred ls else
+                     match arg_0__, arg_1__ with
+                     | _, nil => atEnd
+                     | n, cons _ xs => go (n GHC.Num.- #1) xs
+                     end
+                 end in
+    if n0 GHC.Base.< #0 : bool then atLenPred ls0 else
+    go n0 ls0.
+
+Definition lengthAtLeast {a} : list a -> GHC.Num.Int -> bool :=
+  atLength (GHC.Base.const true) false.
+
+Definition lengthAtMost {a} : list a -> GHC.Num.Int -> bool :=
+  fun lst n =>
+    if n GHC.Base.< #0 : bool then false else
+    atLength Data.Foldable.null true lst n.
+
+Definition lengthIs {a} : list a -> GHC.Num.Int -> bool :=
+  fun lst n =>
+    if n GHC.Base.< #0 : bool then false else
+    atLength Data.Foldable.null false lst n.
+
+Definition lengthLessThan {a} : list a -> GHC.Num.Int -> bool :=
+  atLength (GHC.Base.const false) true.
+
+Definition listLengthCmp {a} : list a -> GHC.Num.Int -> comparison :=
+  let atLen := fun arg_0__ => match arg_0__ with | nil => Eq | _ => Gt end in
+  let atEnd := Lt in atLength atLen atEnd.
+
+Definition capitalise : GHC.Base.String -> GHC.Base.String :=
+  fun arg_0__ => match arg_0__ with | nil => nil | cons c cs => cons c cs end.
+
+Definition changeLast {a} : list a -> a -> list a :=
+  fix changeLast arg_0__ arg_1__
+        := match arg_0__, arg_1__ with
+           | nil, _ => Panic.panic (GHC.Base.hs_string__ "changeLast")
+           | cons _ nil, x => cons x nil
+           | cons x xs, x' => cons x (changeLast xs x')
+           end.
+
+Definition chkAppend {a} : list a -> list a -> list a :=
+  fun xs ys =>
+    if Data.Foldable.null ys : bool then xs else
+    Coq.Init.Datatypes.app xs ys.
+
+Definition cmpList {a}
+   : (a -> a -> comparison) -> list a -> list a -> comparison :=
+  fix cmpList arg_0__ arg_1__ arg_2__
+        := match arg_0__, arg_1__, arg_2__ with
+           | _, nil, nil => Eq
+           | _, nil, _ => Lt
+           | _, _, nil => Gt
+           | cmp, cons a as_, cons b bs =>
+               match cmp a b with
+               | Eq => cmpList cmp as_ bs
+               | xxx => xxx
+               end
+           end.
+
+Definition compareLength {a} {b} : list a -> list b -> comparison :=
+  fix compareLength arg_0__ arg_1__
+        := match arg_0__, arg_1__ with
+           | nil, nil => Eq
+           | cons _ xs, cons _ ys => compareLength xs ys
+           | nil, _ => Lt
+           | _, nil => Gt
+           end.
+
+Definition leLength {a} {b} : list a -> list b -> bool :=
+  fun xs ys =>
+    match compareLength xs ys with
+    | Lt => true
+    | Eq => true
+    | Gt => false
+    end.
+
+Definition ltLength {a} {b} : list a -> list b -> bool :=
+  fun xs ys =>
+    match compareLength xs ys with
+    | Lt => true
+    | Eq => false
+    | Gt => false
+    end.
+
+Definition count {a} : (a -> bool) -> list a -> GHC.Num.Int :=
+  fun p =>
+    let fix go arg_0__ arg_1__
+              := match arg_0__, arg_1__ with
+                 | n, nil => n
+                 | n, cons x xs => if p x : bool then go (n GHC.Num.+ #1) xs else go n xs
+                 end in
+    go #0.
+
+Definition debugIsOn : bool :=
+  false.
+
+Definition dropList {b} {a} : list b -> list a -> list a :=
+  fix dropList arg_0__ arg_1__
+        := match arg_0__, arg_1__ with
+           | nil, xs => xs
+           | _, (nil as xs) => xs
+           | cons _ xs, cons _ ys => dropList xs ys
+           end.
+
+Definition dropTail {a} : GHC.Num.Int -> list a -> list a :=
+  fun n xs =>
+    let fix go arg_0__ arg_1__
+              := match arg_0__, arg_1__ with
+                 | cons _ ys, cons x xs => cons x (go ys xs)
+                 | _, _ => nil
+                 end in
+    go (GHC.List.drop n xs) xs.
+
+Definition dropWhileEndLE {a} : (a -> bool) -> list a -> list a :=
+  fun p =>
+    Data.Foldable.foldr (fun x r =>
+                           if andb (Data.Foldable.null r) (p x) : bool
+                           then nil
+                           else cons x r) nil.
+
+Definition eqListBy {a} : (a -> a -> bool) -> list a -> list a -> bool :=
+  fix eqListBy arg_0__ arg_1__ arg_2__
+        := match arg_0__, arg_1__, arg_2__ with
+           | _, nil, nil => true
+           | eq, cons x xs, cons y ys => andb (eq x y) (eqListBy eq xs ys)
+           | _, _, _ => false
+           end.
+
+Definition eqMaybeBy {a} : (a -> a -> bool) -> option a -> option a -> bool :=
+  fun arg_0__ arg_1__ arg_2__ =>
+    match arg_0__, arg_1__, arg_2__ with
+    | _, None, None => true
+    | eq, Some x, Some y => eq x y
+    | _, _, _ => false
+    end.
+
+Definition equalLength {a} {b} : list a -> list b -> bool :=
+  fix equalLength arg_0__ arg_1__
+        := match arg_0__, arg_1__ with
+           | nil, nil => true
+           | cons _ xs, cons _ ys => equalLength xs ys
+           | _, _ => false
+           end.
+
+Definition exactLog2 : GHC.Num.Integer -> option GHC.Num.Integer :=
+  fun x =>
+    let pow2 :=
+      GHC.DeferredFix.deferredFix1 (fun pow2 x =>
+                                      if x GHC.Base.== #1 : bool then #0 else
+                                      #1 GHC.Num.+ pow2 (Data.Bits.shiftR x #1)) in
+    if (orb (x GHC.Base.<= #0) (x GHC.Base.>= #2147483648)) : bool
+    then None
+    else if (x Data.Bits..&.(**) (GHC.Num.negate x)) GHC.Base./= x : bool
+         then None
+         else Some (pow2 x).
+
+Definition filterByList {a} : list bool -> list a -> list a :=
+  fix filterByList arg_0__ arg_1__
+        := match arg_0__, arg_1__ with
+           | cons true bs, cons x xs => cons x (filterByList bs xs)
+           | cons false bs, cons _ xs => filterByList bs xs
+           | _, _ => nil
+           end.
+
+Definition filterByLists {a} : list bool -> list a -> list a -> list a :=
+  fix filterByLists arg_0__ arg_1__ arg_2__
+        := match arg_0__, arg_1__, arg_2__ with
+           | cons true bs, cons x xs, cons _ ys => cons x (filterByLists bs xs ys)
+           | cons false bs, cons _ xs, cons y ys => cons y (filterByLists bs xs ys)
+           | _, _, _ => nil
+           end.
+
+Definition filterOut {a} : (a -> bool) -> list a -> list a :=
+  fix filterOut arg_0__ arg_1__
+        := match arg_0__, arg_1__ with
+           | _, nil => nil
+           | p, cons x xs => if p x : bool then filterOut p xs else cons x (filterOut p xs)
+           end.
+
+Definition first3M {m} {a} {d} {b} {c} `{GHC.Base.Monad m}
+   : (a -> m d) -> (a * b * c)%type -> m (d * b * c)%type :=
+  fun arg_0__ arg_1__ =>
+    match arg_0__, arg_1__ with
+    | f, pair (pair x y) z => GHC.Base.liftM (fun x' => pair (pair x' y) z) (f x)
+    end.
+
+Definition firstM {m} {a} {c} {b} `{GHC.Base.Monad m}
+   : (a -> m c) -> (a * b)%type -> m (c * b)%type :=
+  fun arg_0__ arg_1__ =>
+    match arg_0__, arg_1__ with
+    | f, pair x y => GHC.Base.liftM (fun x' => pair x' y) (f x)
+    end.
+
+Definition fst3 {a} {d} {b} {c}
+   : (a -> d) -> (a * b * c)%type -> (d * b * c)%type :=
+  fun arg_0__ arg_1__ =>
+    match arg_0__, arg_1__ with
+    | f, pair (pair a b) c => pair (pair (f a) b) c
+    end.
+
+Definition fstOf3 {a} {b} {c} : (a * b * c)%type -> a :=
+  fun arg_0__ => let 'pair (pair a _) _ := arg_0__ in a.
+
+Definition ghciSupported : bool :=
+  false.
+
+Definition ghciTablesNextToCode : bool :=
+  false.
+
+Definition isDarwinHost : bool :=
+  true.
+
+Definition isEqual : comparison -> bool :=
+  fun arg_0__ => match arg_0__ with | Gt => false | Eq => true | Lt => false end.
+
+Definition isIn {a} `{GHC.Base.Eq_ a}
+   : GHC.Base.String -> a -> list a -> bool :=
+  fun _msg x ys => Data.Foldable.elem x ys.
+
+Definition isSingleton {a} : list a -> bool :=
+  fun arg_0__ => match arg_0__ with | cons _ nil => true | _ => false end.
+
+Definition isWindowsHost : bool :=
+  false.
+
+Definition isn'tIn {a} `{GHC.Base.Eq_ a}
+   : GHC.Base.String -> a -> list a -> bool :=
+  fun _msg x ys => Data.Foldable.notElem x ys.
+
+Definition liftFst {a} {b} {c} : (a -> b) -> (a * c)%type -> (b * c)%type :=
+  fun arg_0__ arg_1__ =>
+    match arg_0__, arg_1__ with
+    | f, pair a c => pair (f a) c
+    end.
+
+Definition liftSnd {a} {b} {c} : (a -> b) -> (c * a)%type -> (c * b)%type :=
+  fun arg_0__ arg_1__ =>
+    match arg_0__, arg_1__ with
+    | f, pair c a => pair c (f a)
+    end.
+
+Definition looksLikePackageName : GHC.Base.String -> bool :=
+  fun x => false.
+
+Definition makeRelativeTo
+   : GHC.Base.String -> GHC.Base.String -> GHC.Base.String :=
+  fun this that => this.
+
+Definition mapAndUnzip {a} {b} {c}
+   : (a -> (b * c)%type) -> list a -> (list b * list c)%type :=
+  fix mapAndUnzip arg_0__ arg_1__
+        := match arg_0__, arg_1__ with
+           | _, nil => pair nil nil
+           | f, cons x xs =>
+               let 'pair rs1 rs2 := mapAndUnzip f xs in
+               let 'pair r1 r2 := f x in
+               pair (cons r1 rs1) (cons r2 rs2)
+           end.
+
+Definition mapAndUnzip3 {a} {b} {c} {d}
+   : (a -> (b * c * d)%type) -> list a -> (list b * list c * list d)%type :=
+  fix mapAndUnzip3 arg_0__ arg_1__
+        := match arg_0__, arg_1__ with
+           | _, nil => pair (pair nil nil) nil
+           | f, cons x xs =>
+               let 'pair (pair rs1 rs2) rs3 := mapAndUnzip3 f xs in
+               let 'pair (pair r1 r2) r3 := f x in
+               pair (pair (cons r1 rs1) (cons r2 rs2)) (cons r3 rs3)
+           end.
+
+Definition mapFst {a} {c} {b}
+   : (a -> c) -> list (a * b)%type -> list (c * b)%type :=
+  fun f xys =>
+    let cont_0__ arg_1__ := let 'pair x y := arg_1__ in cons (pair (f x) y) nil in
+    Coq.Lists.List.flat_map cont_0__ xys.
+
+Definition mapSnd {b} {c} {a}
+   : (b -> c) -> list (a * b)%type -> list (a * c)%type :=
+  fun f xys =>
+    let cont_0__ arg_1__ := let 'pair x y := arg_1__ in cons (pair x (f y)) nil in
+    Coq.Lists.List.flat_map cont_0__ xys.
+
+Definition nOfThem {a} : GHC.Num.Int -> a -> list a :=
+  fun n thing => GHC.List.replicate n thing.
+
+Definition ncgDebugIsOn : bool :=
+  false.
+
+Definition neLength {a} {b} : list a -> list b -> bool :=
+  fix neLength arg_0__ arg_1__
+        := match arg_0__, arg_1__ with
+           | nil, nil => false
+           | cons _ xs, cons _ ys => neLength xs ys
+           | _, _ => true
+           end.
+
+Definition notNull {a} : list a -> bool :=
+  fun arg_0__ => match arg_0__ with | nil => false | _ => true end.
+
+Definition lengthExceeds {a} : list a -> GHC.Num.Int -> bool :=
+  fun lst n =>
+    if n GHC.Base.< #0 : bool then true else
+    atLength notNull false lst n.
+
+Definition lengthIsNot {a} : list a -> GHC.Num.Int -> bool :=
+  fun lst n =>
+    if n GHC.Base.< #0 : bool then true else
+    atLength notNull true lst n.
+
+Definition op_zlzazazg__ {f} `{GHC.Base.Applicative f}
+   : f bool -> f bool -> f bool :=
+  GHC.Base.liftA2 andb.
+
+Notation "'_<&&>_'" := (op_zlzazazg__).
+
+Infix "<&&>" := (_<&&>_) (at level 99).
+
+Definition op_zlzbzbzg__ {f} `{GHC.Base.Applicative f}
+   : f bool -> f bool -> f bool :=
+  GHC.Base.liftA2 orb.
+
+Notation "'_<||>_'" := (op_zlzbzbzg__).
+
+Infix "<||>" := (_<||>_) (at level 99).
+
+Definition overrideWith : bool -> OverridingBool -> bool :=
+  fun arg_0__ arg_1__ =>
+    match arg_0__, arg_1__ with
+    | b, Auto => b
+    | _, Always => true
+    | _, Never => false
+    end.
+
+Definition partitionByList {a}
+   : list bool -> list a -> (list a * list a)%type :=
+  let fix go arg_0__ arg_1__ arg_2__ arg_3__
+            := match arg_0__, arg_1__, arg_2__, arg_3__ with
+               | trues, falses, cons true bs, cons x xs => go (cons x trues) falses bs xs
+               | trues, falses, cons false bs, cons x xs => go trues (cons x falses) bs xs
+               | trues, falses, _, _ => pair (GHC.List.reverse trues) (GHC.List.reverse falses)
+               end in
+  go nil nil.
+
+Definition partitionWith {a} {b} {c}
+   : (a -> Data.Either.Either b c) -> list a -> (list b * list c)%type :=
+  fix partitionWith arg_0__ arg_1__
+        := match arg_0__, arg_1__ with
+           | _, nil => pair nil nil
+           | f, cons x xs =>
+               let 'pair bs cs := partitionWith f xs in
+               match f x with
+               | Data.Either.Left b => pair (cons b bs) cs
+               | Data.Either.Right c => pair bs (cons c cs)
+               end
+           end.
+
+Definition seqList {a} {b} : list a -> b -> b :=
+  fix seqList arg_0__ arg_1__
+        := match arg_0__, arg_1__ with
+           | nil, b => b
+           | cons x xs, b => seqList xs b
+           end.
+
+Definition singleton {a} : a -> list a :=
+  fun x => cons x nil.
+
+Definition sizedComplement {bv} `{Data.Bits.Bits bv} : bv -> bv -> bv :=
+  fun vector_mask vect => Data.Bits.xor vector_mask vect.
+
+Definition snd3 {b} {d} {a} {c}
+   : (b -> d) -> (a * b * c)%type -> (a * d * c)%type :=
+  fun arg_0__ arg_1__ =>
+    match arg_0__, arg_1__ with
+    | f, pair (pair a b) c => pair (pair a (f b)) c
+    end.
+
+Definition sndOf3 {a} {b} {c} : (a * b * c)%type -> b :=
+  fun arg_0__ => let 'pair (pair _ b) _ := arg_0__ in b.
+
+Definition snocView {a} : list a -> option (list a * a)%type :=
+  fun arg_0__ =>
+    match arg_0__ with
+    | nil => None
+    | xs =>
+        let fix go arg_1__ arg_2__
+                  := match arg_1__, arg_2__ with
+                     | acc, cons x nil => Some (pair (GHC.List.reverse acc) x)
+                     | acc, cons x xs => go (cons x acc) xs
+                     | _, nil => Panic.panic (GHC.Base.hs_string__ "Util: snocView")
+                     end in
+        go nil xs
+    end.
+
+Definition spanEnd {a} : (a -> bool) -> list a -> (list a * list a)%type :=
+  fun p l =>
+    let fix go arg_0__ arg_1__ arg_2__ arg_3__
+              := match arg_0__, arg_1__, arg_2__, arg_3__ with
+                 | yes, _rev_yes, rev_no, nil => pair yes (GHC.List.reverse rev_no)
+                 | yes, rev_yes, rev_no, cons x xs =>
+                     if p x : bool then go yes (cons x rev_yes) rev_no xs else
+                     go xs nil (cons x (Coq.Init.Datatypes.app rev_yes rev_no)) xs
+                 end in
+    go l nil nil l.
+
+Definition split : GHC.Char.Char -> GHC.Base.String -> list GHC.Base.String :=
+  GHC.DeferredFix.deferredFix2 (fun split c s =>
+                                  let 'pair chunk rest := GHC.List.break (fun arg_0__ => arg_0__ GHC.Base.== c)
+                                                            s in
+                                  match rest with
+                                  | nil => cons chunk nil
+                                  | cons _ rest => cons chunk (split c rest)
+                                  end).
+
+Definition splitAtList {b} {a} : list b -> list a -> (list a * list a)%type :=
+  fix splitAtList arg_0__ arg_1__
+        := match arg_0__, arg_1__ with
+           | nil, xs => pair nil xs
+           | _, (nil as xs) => pair xs xs
+           | cons _ xs, cons y ys =>
+               let 'pair ys' ys'' := splitAtList xs ys in
+               pair (cons y ys') ys''
+           end.
+
+Definition splitEithers {a} {b}
+   : list (Data.Either.Either a b) -> (list a * list b)%type :=
+  fix splitEithers arg_0__
+        := match arg_0__ with
+           | nil => pair nil nil
+           | cons e es =>
+               let 'pair xs ys := splitEithers es in
+               match e with
+               | Data.Either.Left x => pair (cons x xs) ys
+               | Data.Either.Right y => pair xs (cons y ys)
+               end
+           end.
+
+Definition stretchZipWith {a} {b} {c}
+   : (a -> bool) -> b -> (a -> b -> c) -> list a -> list b -> list c :=
+  fix stretchZipWith arg_0__ arg_1__ arg_2__ arg_3__ arg_4__
+        := match arg_0__, arg_1__, arg_2__, arg_3__, arg_4__ with
+           | _, _, _, nil, _ => nil
+           | p, z, f, cons x xs, ys =>
+               if p x : bool then cons (f x z) (stretchZipWith p z f xs ys) else
+               match ys with
+               | nil => nil
+               | cons y ys => cons (f x y) (stretchZipWith p z f xs ys)
+               end
+           end.
+
+Definition takeList {b} {a} : list b -> list a -> list a :=
+  fix takeList arg_0__ arg_1__
+        := match arg_0__, arg_1__ with
+           | nil, _ => nil
+           | cons _ xs, ls =>
+               match ls with
+               | nil => nil
+               | cons y ys => cons y (takeList xs ys)
+               end
+           end.
+
+Definition thdOf3 {a} {b} {c} : (a * b * c)%type -> c :=
+  fun arg_0__ => let 'pair (pair _ _) c := arg_0__ in c.
+
+Definition thenCmp : comparison -> comparison -> comparison :=
+  fun arg_0__ arg_1__ =>
+    match arg_0__, arg_1__ with
+    | Eq, ordering => ordering
+    | ordering, _ => ordering
+    end.
+
+Definition third3 {c} {d} {a} {b}
+   : (c -> d) -> (a * b * c)%type -> (a * b * d)%type :=
+  fun arg_0__ arg_1__ =>
+    match arg_0__, arg_1__ with
+    | f, pair (pair a b) c => pair (pair a b) (f c)
+    end.
+
+Definition transitiveClosure {a}
+   : (a -> list a) -> (a -> a -> bool) -> list a -> list a :=
+  fun succ eq xs =>
+    let fix is_in arg_0__ arg_1__
+              := match arg_0__, arg_1__ with
+                 | _, nil => false
+                 | x, cons y ys => if eq x y : bool then true else is_in x ys
+                 end in
+    let go :=
+      GHC.DeferredFix.deferredFix2 (fun go arg_5__ arg_6__ =>
+                                      match arg_5__, arg_6__ with
+                                      | done, nil => done
+                                      | done, cons x xs =>
+                                          if is_in x done : bool then go done xs else
+                                          go (cons x done) (Coq.Init.Datatypes.app (succ x) xs)
+                                      end) in
+    go nil xs.
+
+Definition uncurry3 {a} {b} {c} {d}
+   : (a -> b -> c -> d) -> (a * b * c)%type -> d :=
+  fun arg_0__ arg_1__ =>
+    match arg_0__, arg_1__ with
+    | f, pair (pair a b) c => f a b c
+    end.
+
+Definition unzipWith {a} {b} {c}
+   : (a -> b -> c) -> list (a * b)%type -> list c :=
+  fun f pairs =>
+    GHC.Base.map (fun arg_0__ => let 'pair a b := arg_0__ in f a b) pairs.
+
+Definition zipEqual {a} {b}
+   : GHC.Base.String -> list a -> list b -> list (a * b)%type :=
+  fun arg_0__ => GHC.List.zip.
+
+Definition zipLazy {a} {b} : list a -> list b -> list (a * b)%type :=
+  fix zipLazy arg_0__ arg_1__
+        := match arg_0__, arg_1__ with
+           | nil, _ => nil
+           | cons x xs, cons y ys => cons (pair x y) (zipLazy xs ys)
+           | _, _ => GHC.Err.patternFailure
+           end.
+
+Definition zipWith3Equal {a} {b} {c} {d}
+   : GHC.Base.String ->
+     (a -> b -> c -> d) -> list a -> list b -> list c -> list d :=
+  fun arg_0__ => GHC.List.zipWith3.
+
+Definition zipWith3Lazy {a} {b} {c} {d}
+   : (a -> b -> c -> d) -> list a -> list b -> list c -> list d :=
+  fix zipWith3Lazy arg_0__ arg_1__ arg_2__ arg_3__
+        := match arg_0__, arg_1__, arg_2__, arg_3__ with
+           | _, nil, _, _ => nil
+           | f, cons a as_, cons b bs, cons c cs =>
+               cons (f a b c) (zipWith3Lazy f as_ bs cs)
+           | _, _, _, _ => GHC.Err.patternFailure
+           end.
+
+Definition zipWith4Equal {a} {b} {c} {d} {e}
+   : GHC.Base.String ->
+     (a -> b -> c -> d -> e) -> list a -> list b -> list c -> list d -> list e :=
+  fun arg_0__ => Data.OldList.zipWith4.
+
+Definition zipWithAndUnzip {a} {b} {c} {d}
+   : (a -> b -> (c * d)%type) -> list a -> list b -> (list c * list d)%type :=
+  fix zipWithAndUnzip arg_0__ arg_1__ arg_2__
+        := match arg_0__, arg_1__, arg_2__ with
+           | f, cons a as_, cons b bs =>
+               let 'pair rs1 rs2 := zipWithAndUnzip f as_ bs in
+               let 'pair r1 r2 := f a b in
+               pair (cons r1 rs1) (cons r2 rs2)
+           | _, _, _ => pair nil nil
+           end.
+
+Definition zipWithEqual {a} {b} {c}
+   : GHC.Base.String -> (a -> b -> c) -> list a -> list b -> list c :=
+  fun arg_0__ => GHC.List.zipWith.
+
+Definition zipWithLazy {a} {b} {c}
+   : (a -> b -> c) -> list a -> list b -> list c :=
+  fix zipWithLazy arg_0__ arg_1__ arg_2__
+        := match arg_0__, arg_1__, arg_2__ with
+           | _, nil, _ => nil
+           | f, cons a as_, cons b bs => cons (f a b) (zipWithLazy f as_ bs)
+           | _, _, _ => GHC.Err.patternFailure
+           end.
+
+Module Notations.
+Notation "'_Util.<&&>_'" := (op_zlzazazg__).
+Infix "Util.<&&>" := (_<&&>_) (at level 99).
+Notation "'_Util.<||>_'" := (op_zlzbzbzg__).
+Infix "Util.<||>" := (_<||>_) (at level 99).
+End Notations.
+
+(* External variables:
+     Eq Gt Lt None Some andb bool comparison cons false list nil op_zt__ option orb
+     pair true unit Coq.Init.Datatypes.app Coq.Lists.List.flat_map Data.Bits.Bits
+     Data.Bits.op_zizazi__ Data.Bits.shiftR Data.Bits.xor Data.Either.Either
+     Data.Either.Left Data.Either.Right Data.Foldable.elem Data.Foldable.foldr
+     Data.Foldable.notElem Data.Foldable.null Data.OldList.zipWith4
+     GHC.Base.Applicative GHC.Base.Eq_ GHC.Base.Monad GHC.Base.String GHC.Base.const
+     GHC.Base.liftA2 GHC.Base.liftM GHC.Base.map GHC.Base.op_zeze__
+     GHC.Base.op_zgze__ GHC.Base.op_zl__ GHC.Base.op_zlze__ GHC.Base.op_zsze__
+     GHC.Char.Char GHC.DeferredFix.deferredFix1 GHC.DeferredFix.deferredFix2
+     GHC.Err.Build_Default GHC.Err.Default GHC.Err.patternFailure GHC.List.break
+     GHC.List.drop GHC.List.replicate GHC.List.reverse GHC.List.zip GHC.List.zipWith
+     GHC.List.zipWith3 GHC.Num.Int GHC.Num.Integer GHC.Num.fromInteger GHC.Num.negate
+     GHC.Num.op_zm__ GHC.Num.op_zp__ Panic.panic
+*)
