examples/ghc/lib/Var.v
@@ -1,0 +1,692 @@
+(* Default settings (from HsToCoq.Coq.Preamble) *)
+
+Generalizable All Variables.
+
+Unset Implicit Arguments.
+Set Maximal Implicit Insertion.
+Unset Strict Implicit.
+Unset Printing Implicit Defensive.
+
+Require Coq.Program.Tactics.
+Require Coq.Program.Wf.
+
+(* Preamble *)
+
+(* Require Import Core.*)
+
+(* Converted imports: *)
+
+Require GHC.Base.
+Require GHC.Err.
+Require GHC.Num.
+Require IdInfo.
+Require Name.
+Require Panic.
+Require Unique.
+Require Util.
+Import GHC.Base.Notations.
+Import GHC.Num.Notations.
+
+(* Converted type declarations: *)
+
+Inductive TyVarBndr tyvar argf : Type
+  := TvBndr : tyvar -> argf -> TyVarBndr tyvar argf.
+
+Inductive ExportFlag : Type
+  := NotExported : ExportFlag
+  |  Exported : ExportFlag.
+
+Inductive IdScope : Type
+  := GlobalId : IdScope
+  |  LocalId : ExportFlag -> IdScope.
+
+Inductive Var : Type
+  := Mk_TyVar : Name.Name -> GHC.Num.Int -> unit -> Var
+  |  Mk_TcTyVar : Name.Name -> GHC.Num.Int -> unit -> unit -> Var
+  |  Mk_Id
+   : Name.Name ->
+     GHC.Num.Int -> unit -> IdScope -> IdInfo.IdDetails -> IdInfo.IdInfo -> Var.
+
+Definition Id :=
+  Var%type.
+
+Definition InId :=
+  Id%type.
+
+Definition JoinId :=
+  Id%type.
+
+Definition NcId :=
+  Id%type.
+
+Definition OutId :=
+  Id%type.
+
+Definition TyCoVar :=
+  Id%type.
+
+Definition InVar :=
+  Var%type.
+
+Definition KindVar :=
+  Var%type.
+
+Definition OutVar :=
+  Var%type.
+
+Definition TKVar :=
+  Var%type.
+
+Definition TyVar :=
+  Var%type.
+
+Definition InTyVar :=
+  TyVar%type.
+
+Definition OutTyVar :=
+  TyVar%type.
+
+Definition TypeVar :=
+  Var%type.
+
+Definition EvId :=
+  Id%type.
+
+Definition EvVar :=
+  EvId%type.
+
+Definition IpId :=
+  EvId%type.
+
+Definition EqVar :=
+  EvId%type.
+
+Definition DictId :=
+  EvId%type.
+
+Definition DFunId :=
+  Id%type.
+
+Definition CoVar :=
+  Id%type.
+
+Definition InCoVar :=
+  CoVar%type.
+
+Definition OutCoVar :=
+  CoVar%type.
+
+Inductive ArgFlag : Type
+  := Required : ArgFlag
+  |  Specified : ArgFlag
+  |  Inferred : ArgFlag.
+
+Definition TyVarBinder :=
+  (TyVarBndr TyVar ArgFlag)%type.
+
+Arguments TvBndr {_} {_} _ _.
+
+Instance Default__ExportFlag : GHC.Err.Default ExportFlag :=
+  GHC.Err.Build_Default _ NotExported.
+
+Instance Default__IdScope : GHC.Err.Default IdScope :=
+  GHC.Err.Build_Default _ GlobalId.
+
+Instance Default__ArgFlag : GHC.Err.Default ArgFlag :=
+  GHC.Err.Build_Default _ Required.
+
+Definition idScope (arg_0__ : Var) :=
+  match arg_0__ with
+  | Mk_TyVar _ _ _ =>
+      GHC.Err.error (GHC.Base.hs_string__
+                     "Partial record selector: field `idScope' has no match in constructor `Mk_TyVar' of type `Var'")
+  | Mk_TcTyVar _ _ _ _ =>
+      GHC.Err.error (GHC.Base.hs_string__
+                     "Partial record selector: field `idScope' has no match in constructor `Mk_TcTyVar' of type `Var'")
+  | Mk_Id _ _ _ idScope _ _ => idScope
+  end.
+
+Definition id_details (arg_0__ : Var) :=
+  match arg_0__ with
+  | Mk_TyVar _ _ _ =>
+      GHC.Err.error (GHC.Base.hs_string__
+                     "Partial record selector: field `id_details' has no match in constructor `Mk_TyVar' of type `Var'")
+  | Mk_TcTyVar _ _ _ _ =>
+      GHC.Err.error (GHC.Base.hs_string__
+                     "Partial record selector: field `id_details' has no match in constructor `Mk_TcTyVar' of type `Var'")
+  | Mk_Id _ _ _ _ id_details _ => id_details
+  end.
+
+Definition id_info (arg_0__ : Var) :=
+  match arg_0__ with
+  | Mk_TyVar _ _ _ =>
+      GHC.Err.error (GHC.Base.hs_string__
+                     "Partial record selector: field `id_info' has no match in constructor `Mk_TyVar' of type `Var'")
+  | Mk_TcTyVar _ _ _ _ =>
+      GHC.Err.error (GHC.Base.hs_string__
+                     "Partial record selector: field `id_info' has no match in constructor `Mk_TcTyVar' of type `Var'")
+  | Mk_Id _ _ _ _ _ id_info => id_info
+  end.
+
+Definition realUnique (arg_0__ : Var) :=
+  match arg_0__ with
+  | Mk_TyVar _ realUnique _ => realUnique
+  | Mk_TcTyVar _ realUnique _ _ => realUnique
+  | Mk_Id _ realUnique _ _ _ _ => realUnique
+  end.
+
+Definition tc_tv_details (arg_0__ : Var) :=
+  match arg_0__ with
+  | Mk_TyVar _ _ _ =>
+      GHC.Err.error (GHC.Base.hs_string__
+                     "Partial record selector: field `tc_tv_details' has no match in constructor `Mk_TyVar' of type `Var'")
+  | Mk_TcTyVar _ _ _ tc_tv_details => tc_tv_details
+  | Mk_Id _ _ _ _ _ _ =>
+      GHC.Err.error (GHC.Base.hs_string__
+                     "Partial record selector: field `tc_tv_details' has no match in constructor `Mk_Id' of type `Var'")
+  end.
+
+Definition varName (arg_0__ : Var) :=
+  match arg_0__ with
+  | Mk_TyVar varName _ _ => varName
+  | Mk_TcTyVar varName _ _ _ => varName
+  | Mk_Id varName _ _ _ _ _ => varName
+  end.
+
+Definition varType (arg_0__ : Var) :=
+  match arg_0__ with
+  | Mk_TyVar _ _ varType => varType
+  | Mk_TcTyVar _ _ varType _ => varType
+  | Mk_Id _ _ varType _ _ _ => varType
+  end.
+(* Midamble *)
+
+Instance Unique_Var : Unique.Uniquable Var := {}.
+Admitted.
+
+Require Import GHC.Err.
+
+
+(*
+Instance Default__IdScope : Default IdScope := Build_Default _ GlobalId. 
+*)
+Instance Default__Var : Default Var := Build_Default _ (Mk_Id default default default default default default).
+
+
+Instance Name_NamedThing_TyCoVar : Name.NamedThing TyCoVar.
+Admitted.
+Instance Name_NamedThing_VarId : Name.NamedThing Id.
+Admitted.
+
+
+(*
+Definition varType (arg_8__ : Var) :=
+  match arg_8__ with
+    | Core.Mk_TyVar _ _ varType => varType
+    | Core.Mk_TcTyVar _ _ varType _ => varType
+    | Core.Mk_Id _ _ varType _ _ _ => varType
+  end.
+
+
+Definition realUnique (arg_8__ : Var) :=
+  match arg_8__ with
+    | Core.Mk_TyVar _ u _ => u
+    | Core.Mk_TcTyVar _ u _ _ => u
+    | Core.Mk_Id _ u _ _ _ _ => u
+  end.
+
+Definition varName (arg_8__ : Var) :=
+  match arg_8__ with
+    | Core.Mk_TyVar n _ _ => n
+    | Core.Mk_TcTyVar n _ _ _ => n
+    | Core.Mk_Id n _ _ _ _ _ => n
+  end.
+*)
+(* Converted value declarations: *)
+
+(* Translating `instance Outputable__TyVarBndr__ArgFlag__11' failed: OOPS!
+   Cannot find information for class Qualified "Outputable" "Outputable"
+   unsupported *)
+
+(* Translating `instance Binary__TyVarBndr' failed: OOPS! Cannot find
+   information for class Qualified "Binary" "Binary" unsupported *)
+
+(* Translating `instance Outputable__ArgFlag' failed: OOPS! Cannot find
+   information for class Qualified "Outputable" "Outputable" unsupported *)
+
+(* Translating `instance Binary__ArgFlag' failed: OOPS! Cannot find information
+   for class Qualified "Binary" "Binary" unsupported *)
+
+(* Translating `instance Outputable__Var' failed: OOPS! Cannot find information
+   for class Qualified "Outputable" "Outputable" unsupported *)
+
+(* Translating `instance NamedThing__Var' failed: OOPS! Cannot find information
+   for class Qualified "Name" "NamedThing" unsupported *)
+
+(* Translating `instance Uniquable__Var' failed: OOPS! Cannot find information
+   for class Qualified "Unique" "Uniquable" unsupported *)
+
+Local Definition Eq___Var_op_zeze__ : Var -> Var -> bool :=
+  fun a b => realUnique a GHC.Base.== realUnique b.
+
+Local Definition Eq___Var_op_zsze__ : Var -> Var -> bool :=
+  fun x y => negb (Eq___Var_op_zeze__ x y).
+
+Program Instance Eq___Var : GHC.Base.Eq_ Var :=
+  fun _ k =>
+    k {| GHC.Base.op_zeze____ := Eq___Var_op_zeze__ ;
+         GHC.Base.op_zsze____ := Eq___Var_op_zsze__ |}.
+
+Local Definition Ord__Var_op_zg__ : Var -> Var -> bool :=
+  fun a b => realUnique a GHC.Base.> realUnique b.
+
+Local Definition Ord__Var_op_zgze__ : Var -> Var -> bool :=
+  fun a b => realUnique a GHC.Base.>= realUnique b.
+
+Local Definition Ord__Var_op_zl__ : Var -> Var -> bool :=
+  fun a b => realUnique a GHC.Base.< realUnique b.
+
+Local Definition Ord__Var_op_zlze__ : Var -> Var -> bool :=
+  fun a b => realUnique a GHC.Base.<= realUnique b.
+
+Local Definition Ord__Var_min : Var -> Var -> Var :=
+  fun x y => if Ord__Var_op_zlze__ x y : bool then x else y.
+
+Local Definition Ord__Var_max : Var -> Var -> Var :=
+  fun x y => if Ord__Var_op_zlze__ x y : bool then y else x.
+
+(* Translating `instance Data__Var' failed: OOPS! Cannot find information for
+   class Qualified "Data.Data" "Data" unsupported *)
+
+(* Translating `instance HasOccName__Var' failed: OOPS! Cannot find information
+   for class Qualified "OccName" "HasOccName" unsupported *)
+
+(* Translating `instance Data__TyVarBndr' failed: OOPS! Cannot find information
+   for class Qualified "Data.Data" "Data" unsupported *)
+
+(* Translating `instance Data__ArgFlag' failed: OOPS! Cannot find information
+   for class Qualified "Data.Data" "Data" unsupported *)
+
+Local Definition Eq___ArgFlag_op_zeze__ : ArgFlag -> ArgFlag -> bool :=
+  fun arg_0__ arg_1__ =>
+    match arg_0__, arg_1__ with
+    | Required, Required => true
+    | Specified, Specified => true
+    | Inferred, Inferred => true
+    | _, _ => false
+    end.
+
+Local Definition Eq___ArgFlag_op_zsze__ : ArgFlag -> ArgFlag -> bool :=
+  fun x y => negb (Eq___ArgFlag_op_zeze__ x y).
+
+Program Instance Eq___ArgFlag : GHC.Base.Eq_ ArgFlag :=
+  fun _ k =>
+    k {| GHC.Base.op_zeze____ := Eq___ArgFlag_op_zeze__ ;
+         GHC.Base.op_zsze____ := Eq___ArgFlag_op_zsze__ |}.
+
+Definition binderArgFlag {tv} {argf} : TyVarBndr tv argf -> argf :=
+  fun arg_0__ => let 'TvBndr _ argf := arg_0__ in argf.
+
+Definition binderVar {tv} {argf} : TyVarBndr tv argf -> tv :=
+  fun arg_0__ => let 'TvBndr v _ := arg_0__ in v.
+
+Definition binderVars {tv} {argf} : list (TyVarBndr tv argf) -> list tv :=
+  fun tvbs => GHC.Base.map binderVar tvbs.
+
+Definition globaliseId : Id -> Id :=
+  fun id =>
+    match id with
+    | Mk_TyVar _ _ _ => GHC.Err.error (GHC.Base.hs_string__ "Partial record update")
+    | Mk_TcTyVar _ _ _ _ =>
+        GHC.Err.error (GHC.Base.hs_string__ "Partial record update")
+    | Mk_Id varName_0__ realUnique_1__ varType_2__ idScope_3__ id_details_4__
+    id_info_5__ =>
+        Mk_Id varName_0__ realUnique_1__ varType_2__ GlobalId id_details_4__ id_info_5__
+    end.
+
+Definition idDetails : Id -> IdInfo.IdDetails :=
+  fun arg_0__ =>
+    match arg_0__ with
+    | Mk_Id _ _ _ _ details _ => details
+    | other =>
+        Panic.panicStr (GHC.Base.hs_string__ "idDetails") (Panic.noString other)
+    end.
+
+Definition idInfo `{Util.HasDebugCallStack} : Id -> IdInfo.IdInfo :=
+  fun arg_0__ =>
+    match arg_0__ with
+    | Mk_Id _ _ _ _ _ info => info
+    | other => Panic.panicStr (GHC.Base.hs_string__ "idInfo") (Panic.noString other)
+    end.
+
+Definition isCoVar : Var -> bool :=
+  fun arg_0__ =>
+    match arg_0__ with
+    | Mk_Id _ _ _ _ details _ => IdInfo.isCoVarDetails details
+    | _ => false
+    end.
+
+Definition isExportedId : Var -> bool :=
+  fun arg_0__ =>
+    match arg_0__ with
+    | Mk_Id _ _ _ GlobalId _ _ => true
+    | Mk_Id _ _ _ (LocalId Exported) _ _ => true
+    | _ => false
+    end.
+
+Definition isGlobalId : Var -> bool :=
+  fun arg_0__ =>
+    match arg_0__ with
+    | Mk_Id _ _ _ GlobalId _ _ => true
+    | _ => false
+    end.
+
+Definition isLocalVar : Var -> bool :=
+  fun v => negb (isGlobalId v).
+
+Definition mustHaveLocalBinding : Var -> bool :=
+  fun var => isLocalVar var.
+
+Definition isId : Var -> bool :=
+  fun arg_0__ => match arg_0__ with | Mk_Id _ _ _ _ _ _ => true | _ => false end.
+
+Definition isLocalId : Var -> bool :=
+  fun arg_0__ =>
+    match arg_0__ with
+    | Mk_Id _ _ _ (LocalId _) _ _ => true
+    | _ => false
+    end.
+
+Definition setIdNotExported : Id -> Id :=
+  fun id =>
+    if andb Util.debugIsOn (negb (isLocalId id)) : bool
+    then (Panic.assertPanic (GHC.Base.hs_string__ "ghc/compiler/basicTypes/Var.hs")
+          #591)
+    else match id with
+         | Mk_TyVar _ _ _ => GHC.Err.error (GHC.Base.hs_string__ "Partial record update")
+         | Mk_TcTyVar _ _ _ _ =>
+             GHC.Err.error (GHC.Base.hs_string__ "Partial record update")
+         | Mk_Id varName_0__ realUnique_1__ varType_2__ idScope_3__ id_details_4__
+         id_info_5__ =>
+             Mk_Id varName_0__ realUnique_1__ varType_2__ (LocalId NotExported)
+                   id_details_4__ id_info_5__
+         end.
+
+Definition isNonCoVarId : Var -> bool :=
+  fun arg_0__ =>
+    match arg_0__ with
+    | Mk_Id _ _ _ _ details _ => negb (IdInfo.isCoVarDetails details)
+    | _ => false
+    end.
+
+Definition isTcTyVar : Var -> bool :=
+  fun arg_0__ => match arg_0__ with | Mk_TcTyVar _ _ _ _ => true | _ => false end.
+
+Definition isTyVar : Var -> bool :=
+  fun arg_0__ =>
+    match arg_0__ with
+    | Mk_TyVar _ _ _ => true
+    | Mk_TcTyVar _ _ _ _ => true
+    | _ => false
+    end.
+
+Definition isTyCoVar : Var -> bool :=
+  fun v => orb (isTyVar v) (isCoVar v).
+
+Definition isVisibleArgFlag : ArgFlag -> bool :=
+  fun arg_0__ => match arg_0__ with | Required => true | _ => false end.
+
+Definition isInvisibleArgFlag : ArgFlag -> bool :=
+  negb GHC.Base.∘ isVisibleArgFlag.
+
+Definition lazySetIdInfo : Id -> IdInfo.IdInfo -> Var :=
+  fun id info =>
+    match id with
+    | Mk_TyVar _ _ _ => GHC.Err.error (GHC.Base.hs_string__ "Partial record update")
+    | Mk_TcTyVar _ _ _ _ =>
+        GHC.Err.error (GHC.Base.hs_string__ "Partial record update")
+    | Mk_Id varName_0__ realUnique_1__ varType_2__ idScope_3__ id_details_4__
+    id_info_5__ =>
+        Mk_Id varName_0__ realUnique_1__ varType_2__ idScope_3__ id_details_4__ info
+    end.
+
+Definition mkTcTyVar : Name.Name -> unit -> unit -> TyVar :=
+  fun name kind details =>
+    Mk_TcTyVar name (Unique.getKey (Name.nameUnique name)) kind details.
+
+Definition mkTyVar : Name.Name -> unit -> TyVar :=
+  fun name kind => Mk_TyVar name (Unique.getKey (Name.nameUnique name)) kind.
+
+Definition mkTyVarBinder : ArgFlag -> Var -> TyVarBinder :=
+  fun vis var => TvBndr var vis.
+
+Definition mkTyVarBinders : ArgFlag -> list TyVar -> list TyVarBinder :=
+  fun vis => GHC.Base.map (mkTyVarBinder vis).
+
+Definition mk_id
+   : Name.Name -> unit -> IdScope -> IdInfo.IdDetails -> IdInfo.IdInfo -> Id :=
+  fun name ty scope details info =>
+    Mk_Id name (Unique.getKey (Name.nameUnique name)) ty scope details info.
+
+Definition mkLocalVar
+   : IdInfo.IdDetails -> Name.Name -> unit -> IdInfo.IdInfo -> Id :=
+  fun details name ty info => mk_id name ty (LocalId NotExported) details info.
+
+Definition mkGlobalVar
+   : IdInfo.IdDetails -> Name.Name -> unit -> IdInfo.IdInfo -> Id :=
+  fun details name ty info => mk_id name ty GlobalId details info.
+
+Definition mkExportedLocalVar
+   : IdInfo.IdDetails -> Name.Name -> unit -> IdInfo.IdInfo -> Id :=
+  fun details name ty info => mk_id name ty (LocalId Exported) details info.
+
+Definition mkCoVar : Name.Name -> unit -> CoVar :=
+  fun name ty =>
+    mk_id name ty (LocalId NotExported) IdInfo.coVarDetails IdInfo.vanillaIdInfo.
+
+Definition sameVis : ArgFlag -> ArgFlag -> bool :=
+  fun arg_0__ arg_1__ =>
+    match arg_0__, arg_1__ with
+    | Required, Required => true
+    | Required, _ => false
+    | _, Required => false
+    | _, _ => true
+    end.
+
+Definition setIdDetails : Id -> IdInfo.IdDetails -> Id :=
+  fun id details =>
+    match id with
+    | Mk_TyVar _ _ _ => GHC.Err.error (GHC.Base.hs_string__ "Partial record update")
+    | Mk_TcTyVar _ _ _ _ =>
+        GHC.Err.error (GHC.Base.hs_string__ "Partial record update")
+    | Mk_Id varName_0__ realUnique_1__ varType_2__ idScope_3__ id_details_4__
+    id_info_5__ =>
+        Mk_Id varName_0__ realUnique_1__ varType_2__ idScope_3__ details id_info_5__
+    end.
+
+Definition setIdExported : Id -> Id :=
+  fun arg_0__ =>
+    match arg_0__ with
+    | (Mk_Id _ _ _ (LocalId _) _ _ as id) =>
+        match id with
+        | Mk_TyVar _ _ _ => GHC.Err.error (GHC.Base.hs_string__ "Partial record update")
+        | Mk_TcTyVar _ _ _ _ =>
+            GHC.Err.error (GHC.Base.hs_string__ "Partial record update")
+        | Mk_Id varName_1__ realUnique_2__ varType_3__ idScope_4__ id_details_5__
+        id_info_6__ =>
+            Mk_Id varName_1__ realUnique_2__ varType_3__ (LocalId Exported) id_details_5__
+                  id_info_6__
+        end
+    | (Mk_Id _ _ _ GlobalId _ _ as id) => id
+    | tv =>
+        Panic.panicStr (GHC.Base.hs_string__ "setIdExported") (Panic.noString tv)
+    end.
+
+Definition setTcTyVarDetails : TyVar -> unit -> TyVar :=
+  fun tv details =>
+    match tv with
+    | Mk_TyVar _ _ _ => GHC.Err.error (GHC.Base.hs_string__ "Partial record update")
+    | Mk_TcTyVar varName_0__ realUnique_1__ varType_2__ tc_tv_details_3__ =>
+        Mk_TcTyVar varName_0__ realUnique_1__ varType_2__ details
+    | Mk_Id _ _ _ _ _ _ =>
+        GHC.Err.error (GHC.Base.hs_string__ "Partial record update")
+    end.
+
+Definition setTyVarKind : TyVar -> unit -> TyVar :=
+  fun tv k =>
+    match tv with
+    | Mk_TyVar varName_0__ realUnique_1__ varType_2__ =>
+        Mk_TyVar varName_0__ realUnique_1__ k
+    | Mk_TcTyVar varName_3__ realUnique_4__ varType_5__ tc_tv_details_6__ =>
+        Mk_TcTyVar varName_3__ realUnique_4__ k tc_tv_details_6__
+    | Mk_Id varName_7__ realUnique_8__ varType_9__ idScope_10__ id_details_11__
+    id_info_12__ =>
+        Mk_Id varName_7__ realUnique_8__ k idScope_10__ id_details_11__ id_info_12__
+    end.
+
+Definition setVarName : Var -> Name.Name -> Var :=
+  fun var new_name =>
+    match var with
+    | Mk_TyVar varName_0__ realUnique_1__ varType_2__ =>
+        Mk_TyVar new_name (Unique.getKey (Unique.getUnique new_name)) varType_2__
+    | Mk_TcTyVar varName_3__ realUnique_4__ varType_5__ tc_tv_details_6__ =>
+        Mk_TcTyVar new_name (Unique.getKey (Unique.getUnique new_name)) varType_5__
+                   tc_tv_details_6__
+    | Mk_Id varName_7__ realUnique_8__ varType_9__ idScope_10__ id_details_11__
+    id_info_12__ =>
+        Mk_Id new_name (Unique.getKey (Unique.getUnique new_name)) varType_9__
+              idScope_10__ id_details_11__ id_info_12__
+    end.
+
+Definition setTyVarName : TyVar -> Name.Name -> TyVar :=
+  setVarName.
+
+Definition setVarType : Id -> unit -> Id :=
+  fun id ty =>
+    match id with
+    | Mk_TyVar varName_0__ realUnique_1__ varType_2__ =>
+        Mk_TyVar varName_0__ realUnique_1__ ty
+    | Mk_TcTyVar varName_3__ realUnique_4__ varType_5__ tc_tv_details_6__ =>
+        Mk_TcTyVar varName_3__ realUnique_4__ ty tc_tv_details_6__
+    | Mk_Id varName_7__ realUnique_8__ varType_9__ idScope_10__ id_details_11__
+    id_info_12__ =>
+        Mk_Id varName_7__ realUnique_8__ ty idScope_10__ id_details_11__ id_info_12__
+    end.
+
+Definition setVarUnique : Var -> Unique.Unique -> Var :=
+  fun var uniq =>
+    match var with
+    | Mk_TyVar varName_0__ realUnique_1__ varType_2__ =>
+        Mk_TyVar (Name.setNameUnique (varName var) uniq) (Unique.getKey uniq)
+                 varType_2__
+    | Mk_TcTyVar varName_3__ realUnique_4__ varType_5__ tc_tv_details_6__ =>
+        Mk_TcTyVar (Name.setNameUnique (varName var) uniq) (Unique.getKey uniq)
+                   varType_5__ tc_tv_details_6__
+    | Mk_Id varName_7__ realUnique_8__ varType_9__ idScope_10__ id_details_11__
+    id_info_12__ =>
+        Mk_Id (Name.setNameUnique (varName var) uniq) (Unique.getKey uniq) varType_9__
+              idScope_10__ id_details_11__ id_info_12__
+    end.
+
+Definition setTyVarUnique : TyVar -> Unique.Unique -> TyVar :=
+  setVarUnique.
+
+Definition tcTyVarDetails : TyVar -> unit :=
+  fun x => tt.
+
+Definition tyVarKind : TyVar -> unit :=
+  varType.
+
+Definition updateTyVarKind : (unit -> unit) -> TyVar -> TyVar :=
+  fun update tv =>
+    match tv with
+    | Mk_TyVar varName_0__ realUnique_1__ varType_2__ =>
+        Mk_TyVar varName_0__ realUnique_1__ (update (tyVarKind tv))
+    | Mk_TcTyVar varName_3__ realUnique_4__ varType_5__ tc_tv_details_6__ =>
+        Mk_TcTyVar varName_3__ realUnique_4__ (update (tyVarKind tv)) tc_tv_details_6__
+    | Mk_Id varName_7__ realUnique_8__ varType_9__ idScope_10__ id_details_11__
+    id_info_12__ =>
+        Mk_Id varName_7__ realUnique_8__ (update (tyVarKind tv)) idScope_10__
+              id_details_11__ id_info_12__
+    end.
+
+Definition updateTyVarKindM {m} `{(GHC.Base.Monad m)}
+   : (unit -> m unit) -> TyVar -> m TyVar :=
+  fun update tv =>
+    update (tyVarKind tv) GHC.Base.>>=
+    (fun k' =>
+       GHC.Base.return_ (match tv with
+                         | Mk_TyVar varName_0__ realUnique_1__ varType_2__ =>
+                             Mk_TyVar varName_0__ realUnique_1__ k'
+                         | Mk_TcTyVar varName_3__ realUnique_4__ varType_5__ tc_tv_details_6__ =>
+                             Mk_TcTyVar varName_3__ realUnique_4__ k' tc_tv_details_6__
+                         | Mk_Id varName_7__ realUnique_8__ varType_9__ idScope_10__ id_details_11__
+                         id_info_12__ =>
+                             Mk_Id varName_7__ realUnique_8__ k' idScope_10__ id_details_11__ id_info_12__
+                         end)).
+
+Definition binderKind {argf} : TyVarBndr TyVar argf -> unit :=
+  fun arg_0__ => let 'TvBndr tv _ := arg_0__ in tyVarKind tv.
+
+Definition tyVarName : TyVar -> Name.Name :=
+  varName.
+
+Definition updateVarType : (unit -> unit) -> Id -> Id :=
+  fun f id =>
+    match id with
+    | Mk_TyVar varName_0__ realUnique_1__ varType_2__ =>
+        Mk_TyVar varName_0__ realUnique_1__ (f (varType id))
+    | Mk_TcTyVar varName_3__ realUnique_4__ varType_5__ tc_tv_details_6__ =>
+        Mk_TcTyVar varName_3__ realUnique_4__ (f (varType id)) tc_tv_details_6__
+    | Mk_Id varName_7__ realUnique_8__ varType_9__ idScope_10__ id_details_11__
+    id_info_12__ =>
+        Mk_Id varName_7__ realUnique_8__ (f (varType id)) idScope_10__ id_details_11__
+              id_info_12__
+    end.
+
+Definition updateVarTypeM {m} `{GHC.Base.Monad m}
+   : (unit -> m unit) -> Id -> m Id :=
+  fun f id =>
+    f (varType id) GHC.Base.>>=
+    (fun ty' =>
+       GHC.Base.return_ (match id with
+                         | Mk_TyVar varName_0__ realUnique_1__ varType_2__ =>
+                             Mk_TyVar varName_0__ realUnique_1__ ty'
+                         | Mk_TcTyVar varName_3__ realUnique_4__ varType_5__ tc_tv_details_6__ =>
+                             Mk_TcTyVar varName_3__ realUnique_4__ ty' tc_tv_details_6__
+                         | Mk_Id varName_7__ realUnique_8__ varType_9__ idScope_10__ id_details_11__
+                         id_info_12__ =>
+                             Mk_Id varName_7__ realUnique_8__ ty' idScope_10__ id_details_11__ id_info_12__
+                         end)).
+
+Definition varUnique : Var -> Unique.Unique :=
+  fun var => Unique.mkUniqueGrimily (realUnique var).
+
+Definition nonDetCmpVar : Var -> Var -> comparison :=
+  fun a b => Unique.nonDetCmpUnique (varUnique a) (varUnique b).
+
+Local Definition Ord__Var_compare : Var -> Var -> comparison :=
+  fun a b => nonDetCmpVar a b.
+
+Program Instance Ord__Var : GHC.Base.Ord Var :=
+  fun _ k =>
+    k {| GHC.Base.op_zl____ := Ord__Var_op_zl__ ;
+         GHC.Base.op_zlze____ := Ord__Var_op_zlze__ ;
+         GHC.Base.op_zg____ := Ord__Var_op_zg__ ;
+         GHC.Base.op_zgze____ := Ord__Var_op_zgze__ ;
+         GHC.Base.compare__ := Ord__Var_compare ;
+         GHC.Base.max__ := Ord__Var_max ;
+         GHC.Base.min__ := Ord__Var_min |}.
+
+(* External variables:
+     andb bool comparison false list negb orb true tt unit GHC.Base.Eq_
+     GHC.Base.Monad GHC.Base.Ord GHC.Base.map GHC.Base.op_z2218U__ GHC.Base.op_zeze__
+     GHC.Base.op_zg__ GHC.Base.op_zgze__ GHC.Base.op_zgzgze__ GHC.Base.op_zl__
+     GHC.Base.op_zlze__ GHC.Base.return_ GHC.Err.Build_Default GHC.Err.Default
+     GHC.Err.error GHC.Num.Int GHC.Num.fromInteger IdInfo.IdDetails IdInfo.IdInfo
+     IdInfo.coVarDetails IdInfo.isCoVarDetails IdInfo.vanillaIdInfo Name.Name
+     Name.nameUnique Name.setNameUnique Panic.assertPanic Panic.noString
+     Panic.panicStr Unique.Unique Unique.getKey Unique.getUnique
+     Unique.mkUniqueGrimily Unique.nonDetCmpUnique Util.HasDebugCallStack
+     Util.debugIsOn
+*)
