examples/ghc/lib/VarEnv.v
@@ -1,0 +1,609 @@
+(* Default settings (from HsToCoq.Coq.Preamble) *)
+
+Generalizable All Variables.
+
+Unset Implicit Arguments.
+Set Maximal Implicit Insertion.
+Unset Strict Implicit.
+Unset Printing Implicit Defensive.
+
+Require Coq.Program.Tactics.
+Require Coq.Program.Wf.
+
+(* Preamble *)
+
+
+
+(* Converted imports: *)
+
+Require Data.Foldable.
+Require Data.Tuple.
+Require GHC.Base.
+Require GHC.DeferredFix.
+Require GHC.Err.
+Require GHC.Num.
+Require Maybes.
+Require OccName.
+Require Panic.
+Require UniqDFM.
+Require UniqFM.
+Require UniqSet.
+Require Unique.
+Require Util.
+Require Var.
+Require VarSet.
+Import GHC.Base.Notations.
+Import GHC.Num.Notations.
+
+(* Converted type declarations: *)
+
+Definition VarEnv :=
+  UniqFM.UniqFM%type.
+
+Definition TyVarEnv :=
+  VarEnv%type.
+
+Definition TyCoVarEnv :=
+  VarEnv%type.
+
+Definition TidyEnv :=
+  (OccName.TidyOccEnv * VarEnv Var.Var)%type%type.
+
+Inductive InScopeSet : Type
+  := InScope : VarSet.VarSet -> GHC.Num.Int -> InScopeSet.
+
+Inductive RnEnv2 : Type
+  := RV2 : VarEnv Var.Var -> VarEnv Var.Var -> InScopeSet -> RnEnv2.
+
+Definition IdEnv :=
+  VarEnv%type.
+
+Definition DVarEnv :=
+  UniqDFM.UniqDFM%type.
+
+Definition DTyVarEnv :=
+  DVarEnv%type.
+
+Definition DIdEnv :=
+  DVarEnv%type.
+
+Definition CoVarEnv :=
+  VarEnv%type.
+
+Definition envL (arg_0__ : RnEnv2) :=
+  let 'RV2 envL _ _ := arg_0__ in
+  envL.
+
+Definition envR (arg_0__ : RnEnv2) :=
+  let 'RV2 _ envR _ := arg_0__ in
+  envR.
+
+Definition in_scope (arg_0__ : RnEnv2) :=
+  let 'RV2 _ _ in_scope := arg_0__ in
+  in_scope.
+(* Midamble *)
+
+(*Axiom uniqAway' : InScopeSet -> Core.Var -> Core.Var.
+  fun arg_55__ arg_56__ =>
+    match arg_55__ , arg_56__ with
+      | InScope set n , var =>
+        let orig_unique := Unique.getUnique var in
+        let try :=
+            fix try k
+              := let uniq := Unique.deriveUnique orig_unique (n GHC.Num.* k) in
+                 if VarSet.elemVarSetByKey uniq set : bool
+                 then try (k GHC.Num.+ GHC.Num.fromInteger 1)
+                 else Var.setVarUnique var uniq in
+        try (GHC.Num.fromInteger 1)
+    end.
+*)
+
+Require GHC.Err.
+
+Instance Default__InScopeSet : GHC.Err.Default InScopeSet :=
+  GHC.Err.Build_Default _ (InScope GHC.Err.default GHC.Err.default).
+Instance Default__RnEnv2 : GHC.Err.Default RnEnv2 :=
+  GHC.Err.Build_Default _ (RV2 GHC.Err.default GHC.Err.default GHC.Err.default).
+Instance Default__TidyEnv : GHC.Err.Default TidyEnv.
+Admitted.
+
+
+(* needs UniqFM.plusUFM_CD *)
+Parameter plusVarEnv_CD : forall {a}, (a -> a -> a) -> VarEnv a -> a -> VarEnv
+                               a -> a -> VarEnv a.
+
+(* Converted value declarations: *)
+
+(* Translating `instance Outputable__InScopeSet' failed: OOPS! Cannot find
+   information for class Qualified "Outputable" "Outputable" unsupported *)
+
+Definition alterDVarEnv {a}
+   : (option a -> option a) -> DVarEnv a -> Var.Var -> DVarEnv a :=
+  UniqDFM.alterUDFM.
+
+Definition alterVarEnv {a}
+   : (option a -> option a) -> VarEnv a -> Var.Var -> VarEnv a :=
+  UniqFM.alterUFM.
+
+Definition anyDVarEnv {a} : (a -> bool) -> DVarEnv a -> bool :=
+  UniqDFM.anyUDFM.
+
+Definition dVarEnvElts {a} : DVarEnv a -> list a :=
+  UniqDFM.eltsUDFM.
+
+Definition delDVarEnv {a} : DVarEnv a -> Var.Var -> DVarEnv a :=
+  UniqDFM.delFromUDFM.
+
+Definition delDVarEnvList {a} : DVarEnv a -> list Var.Var -> DVarEnv a :=
+  UniqDFM.delListFromUDFM.
+
+Definition delInScopeSet : InScopeSet -> Var.Var -> InScopeSet :=
+  fun arg_0__ arg_1__ =>
+    match arg_0__, arg_1__ with
+    | InScope in_scope n, v => InScope (VarSet.delVarSet in_scope v) n
+    end.
+
+Definition delVarEnv {a} : VarEnv a -> Var.Var -> VarEnv a :=
+  UniqFM.delFromUFM.
+
+Definition delVarEnvList {a} : VarEnv a -> list Var.Var -> VarEnv a :=
+  UniqFM.delListFromUFM.
+
+Definition delVarEnv_Directly {a} : VarEnv a -> Unique.Unique -> VarEnv a :=
+  UniqFM.delFromUFM_Directly.
+
+Definition disjointVarEnv {a} : VarEnv a -> VarEnv a -> bool :=
+  UniqFM.disjointUFM.
+
+Definition elemDVarEnv {a} : Var.Var -> DVarEnv a -> bool :=
+  UniqDFM.elemUDFM.
+
+Definition elemInScopeSet : Var.Var -> InScopeSet -> bool :=
+  fun arg_0__ arg_1__ =>
+    match arg_0__, arg_1__ with
+    | v, InScope in_scope _ => VarSet.elemVarSet v in_scope
+    end.
+
+Definition rnInScope : Var.Var -> RnEnv2 -> bool :=
+  fun x env => elemInScopeSet x (in_scope env).
+
+Definition elemVarEnv {a} : Var.Var -> VarEnv a -> bool :=
+  UniqFM.elemUFM.
+
+Definition inRnEnvL : RnEnv2 -> Var.Var -> bool :=
+  fun arg_0__ arg_1__ =>
+    match arg_0__, arg_1__ with
+    | RV2 env _ _, v => elemVarEnv v env
+    end.
+
+Definition inRnEnvR : RnEnv2 -> Var.Var -> bool :=
+  fun arg_0__ arg_1__ =>
+    match arg_0__, arg_1__ with
+    | RV2 _ env _, v => elemVarEnv v env
+    end.
+
+Definition elemVarEnvByKey {a} : Unique.Unique -> VarEnv a -> bool :=
+  UniqFM.elemUFM_Directly.
+
+Definition emptyDVarEnv {a} : DVarEnv a :=
+  UniqDFM.emptyUDFM.
+
+Definition emptyInScopeSet : InScopeSet :=
+  InScope VarSet.emptyVarSet #1.
+
+Definition emptyVarEnv {a} : VarEnv a :=
+  UniqFM.emptyUFM.
+
+Definition mkRnEnv2 : InScopeSet -> RnEnv2 :=
+  fun vars => RV2 emptyVarEnv emptyVarEnv vars.
+
+Definition nukeRnEnvL : RnEnv2 -> RnEnv2 :=
+  fun env =>
+    let 'RV2 envL_0__ envR_1__ in_scope_2__ := env in
+    RV2 emptyVarEnv envR_1__ in_scope_2__.
+
+Definition nukeRnEnvR : RnEnv2 -> RnEnv2 :=
+  fun env =>
+    let 'RV2 envL_0__ envR_1__ in_scope_2__ := env in
+    RV2 envL_0__ emptyVarEnv in_scope_2__.
+
+Definition emptyTidyEnv : TidyEnv :=
+  pair OccName.emptyTidyOccEnv emptyVarEnv.
+
+Definition extendDVarEnv {a} : DVarEnv a -> Var.Var -> a -> DVarEnv a :=
+  UniqDFM.addToUDFM.
+
+Definition extendDVarEnvList {a}
+   : DVarEnv a -> list (Var.Var * a)%type -> DVarEnv a :=
+  UniqDFM.addListToUDFM.
+
+Definition extendDVarEnv_C {a}
+   : (a -> a -> a) -> DVarEnv a -> Var.Var -> a -> DVarEnv a :=
+  UniqDFM.addToUDFM_C.
+
+Definition extendInScopeSet : InScopeSet -> Var.Var -> InScopeSet :=
+  fun arg_0__ arg_1__ =>
+    match arg_0__, arg_1__ with
+    | InScope in_scope n, v =>
+        InScope (VarSet.extendVarSet in_scope v) (n GHC.Num.+ #1)
+    end.
+
+Definition delBndrR : RnEnv2 -> Var.Var -> RnEnv2 :=
+  fun arg_0__ arg_1__ =>
+    match arg_0__, arg_1__ with
+    | (RV2 _ env in_scope as rn), v =>
+        let 'RV2 envL_2__ envR_3__ in_scope_4__ := rn in
+        RV2 envL_2__ (delVarEnv env v) (extendInScopeSet in_scope v)
+    end.
+
+Definition delBndrL : RnEnv2 -> Var.Var -> RnEnv2 :=
+  fun arg_0__ arg_1__ =>
+    match arg_0__, arg_1__ with
+    | (RV2 env _ in_scope as rn), v =>
+        let 'RV2 envL_2__ envR_3__ in_scope_4__ := rn in
+        RV2 (delVarEnv env v) envR_3__ (extendInScopeSet in_scope v)
+    end.
+
+Definition extendInScopeSetList : InScopeSet -> list Var.Var -> InScopeSet :=
+  fun arg_0__ arg_1__ =>
+    match arg_0__, arg_1__ with
+    | InScope in_scope n, vs =>
+        InScope (Data.Foldable.foldl (fun s v => VarSet.extendVarSet s v) in_scope vs)
+        (n GHC.Num.+ Data.Foldable.length vs)
+    end.
+
+Definition delBndrsR : RnEnv2 -> list Var.Var -> RnEnv2 :=
+  fun arg_0__ arg_1__ =>
+    match arg_0__, arg_1__ with
+    | (RV2 _ env in_scope as rn), v =>
+        let 'RV2 envL_2__ envR_3__ in_scope_4__ := rn in
+        RV2 envL_2__ (delVarEnvList env v) (extendInScopeSetList in_scope v)
+    end.
+
+Definition delBndrsL : RnEnv2 -> list Var.Var -> RnEnv2 :=
+  fun arg_0__ arg_1__ =>
+    match arg_0__, arg_1__ with
+    | (RV2 env _ in_scope as rn), v =>
+        let 'RV2 envL_2__ envR_3__ in_scope_4__ := rn in
+        RV2 (delVarEnvList env v) envR_3__ (extendInScopeSetList in_scope v)
+    end.
+
+Definition extendInScopeSetSet : InScopeSet -> VarSet.VarSet -> InScopeSet :=
+  fun arg_0__ arg_1__ =>
+    match arg_0__, arg_1__ with
+    | InScope in_scope n, vs =>
+        InScope (VarSet.unionVarSet in_scope vs) (n GHC.Num.+ UniqSet.sizeUniqSet vs)
+    end.
+
+Definition addRnInScopeSet : RnEnv2 -> VarSet.VarSet -> RnEnv2 :=
+  fun env vs =>
+    if VarSet.isEmptyVarSet vs : bool then env else
+    let 'RV2 envL_0__ envR_1__ in_scope_2__ := env in
+    RV2 envL_0__ envR_1__ (extendInScopeSetSet (in_scope env) vs).
+
+Definition extendVarEnv {a} : VarEnv a -> Var.Var -> a -> VarEnv a :=
+  UniqFM.addToUFM.
+
+Definition extendVarEnvList {a}
+   : VarEnv a -> list (Var.Var * a)%type -> VarEnv a :=
+  UniqFM.addListToUFM.
+
+Definition extendVarEnv_Acc {a} {b}
+   : (a -> b -> b) -> (a -> b) -> VarEnv b -> Var.Var -> a -> VarEnv b :=
+  UniqFM.addToUFM_Acc.
+
+Definition extendVarEnv_C {a}
+   : (a -> a -> a) -> VarEnv a -> Var.Var -> a -> VarEnv a :=
+  UniqFM.addToUFM_C.
+
+Definition extendVarEnv_Directly {a}
+   : VarEnv a -> Unique.Unique -> a -> VarEnv a :=
+  UniqFM.addToUFM_Directly.
+
+Definition filterDVarEnv {a} : (a -> bool) -> DVarEnv a -> DVarEnv a :=
+  UniqDFM.filterUDFM.
+
+Definition filterVarEnv {a} : (a -> bool) -> VarEnv a -> VarEnv a :=
+  UniqFM.filterUFM.
+
+Definition filterVarEnv_Directly {a}
+   : (Unique.Unique -> a -> bool) -> VarEnv a -> VarEnv a :=
+  UniqFM.filterUFM_Directly.
+
+Definition restrictVarEnv {a} : VarEnv a -> VarSet.VarSet -> VarEnv a :=
+  fun env vs =>
+    let keep :=
+      fun arg_0__ arg_1__ =>
+        match arg_0__, arg_1__ with
+        | u, _ => VarSet.elemVarSetByKey u vs
+        end in
+    filterVarEnv_Directly keep env.
+
+Definition foldDVarEnv {a} {b} : (a -> b -> b) -> b -> DVarEnv a -> b :=
+  UniqDFM.foldUDFM.
+
+Definition getInScopeVars : InScopeSet -> VarSet.VarSet :=
+  fun arg_0__ => let 'InScope vs _ := arg_0__ in vs.
+
+Definition isEmptyDVarEnv {a} : DVarEnv a -> bool :=
+  UniqDFM.isNullUDFM.
+
+Definition isEmptyVarEnv {a} : VarEnv a -> bool :=
+  UniqFM.isNullUFM.
+
+Definition intersectsVarEnv {a} : VarEnv a -> VarEnv a -> bool :=
+  fun e1 e2 => negb (isEmptyVarEnv (UniqFM.intersectUFM e1 e2)).
+
+Definition lookupDVarEnv {a} : DVarEnv a -> Var.Var -> option a :=
+  UniqDFM.lookupUDFM.
+
+Definition modifyDVarEnv {a} : (a -> a) -> DVarEnv a -> Var.Var -> DVarEnv a :=
+  fun mangle_fn env key =>
+    match (lookupDVarEnv env key) with
+    | None => env
+    | Some xx => extendDVarEnv env key (mangle_fn xx)
+    end.
+
+Definition lookupInScope : InScopeSet -> Var.Var -> option Var.Var :=
+  fun arg_0__ arg_1__ =>
+    match arg_0__, arg_1__ with
+    | InScope in_scope _, v => VarSet.lookupVarSet in_scope v
+    end.
+
+Definition lookupRnInScope : RnEnv2 -> Var.Var -> Var.Var :=
+  fun env v => Maybes.orElse (lookupInScope (in_scope env) v) v.
+
+Definition lookupInScope_Directly
+   : InScopeSet -> Unique.Unique -> option Var.Var :=
+  fun arg_0__ arg_1__ =>
+    match arg_0__, arg_1__ with
+    | InScope in_scope _, uniq => VarSet.lookupVarSet_Directly in_scope uniq
+    end.
+
+Definition lookupVarEnv {a} : VarEnv a -> Var.Var -> option a :=
+  UniqFM.lookupUFM.
+
+Definition rnOccL : RnEnv2 -> Var.Var -> Var.Var :=
+  fun arg_0__ arg_1__ =>
+    match arg_0__, arg_1__ with
+    | RV2 env _ _, v => Maybes.orElse (lookupVarEnv env v) v
+    end.
+
+Definition rnOccL_maybe : RnEnv2 -> Var.Var -> option Var.Var :=
+  fun arg_0__ arg_1__ =>
+    match arg_0__, arg_1__ with
+    | RV2 env _ _, v => lookupVarEnv env v
+    end.
+
+Definition rnOccR : RnEnv2 -> Var.Var -> Var.Var :=
+  fun arg_0__ arg_1__ =>
+    match arg_0__, arg_1__ with
+    | RV2 _ env _, v => Maybes.orElse (lookupVarEnv env v) v
+    end.
+
+Definition rnOccR_maybe : RnEnv2 -> Var.Var -> option Var.Var :=
+  fun arg_0__ arg_1__ =>
+    match arg_0__, arg_1__ with
+    | RV2 _ env _, v => lookupVarEnv env v
+    end.
+
+Definition modifyVarEnv {a} : (a -> a) -> VarEnv a -> Var.Var -> VarEnv a :=
+  fun mangle_fn env key =>
+    match (lookupVarEnv env key) with
+    | None => env
+    | Some xx => extendVarEnv env key (mangle_fn xx)
+    end.
+
+Definition lookupVarEnv_Directly {a} : VarEnv a -> Unique.Unique -> option a :=
+  UniqFM.lookupUFM_Directly.
+
+Definition lookupVarEnv_NF {a} `{_ : GHC.Err.Default a} (env : VarEnv a) id
+   : a :=
+  match lookupVarEnv env id with
+  | Some xx => xx
+  | None => GHC.Err.default
+  end.
+
+Definition lookupWithDefaultVarEnv {a} : VarEnv a -> a -> Var.Var -> a :=
+  UniqFM.lookupWithDefaultUFM.
+
+Definition mapDVarEnv {a} {b} : (a -> b) -> DVarEnv a -> DVarEnv b :=
+  UniqDFM.mapUDFM.
+
+Definition mapVarEnv {a} {b} : (a -> b) -> VarEnv a -> VarEnv b :=
+  UniqFM.mapUFM.
+
+Definition minusDVarEnv {a} {a'} : DVarEnv a -> DVarEnv a' -> DVarEnv a :=
+  UniqDFM.minusUDFM.
+
+Definition minusVarEnv {a} {b} : VarEnv a -> VarEnv b -> VarEnv a :=
+  UniqFM.minusUFM.
+
+Definition mkDVarEnv {a} : list (Var.Var * a)%type -> DVarEnv a :=
+  UniqDFM.listToUDFM.
+
+Definition mkInScopeSet : VarSet.VarSet -> InScopeSet :=
+  fun in_scope => InScope in_scope #1.
+
+Definition mkVarEnv {a} : list (Var.Var * a)%type -> VarEnv a :=
+  UniqFM.listToUFM.
+
+Definition zipVarEnv {a} : list Var.Var -> list a -> VarEnv a :=
+  fun tyvars tys =>
+    mkVarEnv (Util.zipEqual (GHC.Base.hs_string__ "zipVarEnv") tyvars tys).
+
+Definition mkVarEnv_Directly {a} : list (Unique.Unique * a)%type -> VarEnv a :=
+  UniqFM.listToUFM_Directly.
+
+Definition modifyVarEnv_Directly {a}
+   : (a -> a) -> UniqFM.UniqFM a -> Unique.Unique -> UniqFM.UniqFM a :=
+  fun mangle_fn env key =>
+    match (UniqFM.lookupUFM_Directly env key) with
+    | None => env
+    | Some xx => UniqFM.addToUFM_Directly env key (mangle_fn xx)
+    end.
+
+Definition partitionDVarEnv {a}
+   : (a -> bool) -> DVarEnv a -> (DVarEnv a * DVarEnv a)%type :=
+  UniqDFM.partitionUDFM.
+
+Definition partitionVarEnv {a}
+   : (a -> bool) -> VarEnv a -> (VarEnv a * VarEnv a)%type :=
+  UniqFM.partitionUFM.
+
+Definition plusDVarEnv {a} : DVarEnv a -> DVarEnv a -> DVarEnv a :=
+  UniqDFM.plusUDFM.
+
+Definition plusDVarEnv_C {a}
+   : (a -> a -> a) -> DVarEnv a -> DVarEnv a -> DVarEnv a :=
+  UniqDFM.plusUDFM_C.
+
+Definition plusMaybeVarEnv_C {a}
+   : (a -> a -> option a) -> VarEnv a -> VarEnv a -> VarEnv a :=
+  UniqFM.plusMaybeUFM_C.
+
+Definition plusVarEnv {a} : VarEnv a -> VarEnv a -> VarEnv a :=
+  UniqFM.plusUFM.
+
+Definition plusVarEnvList {a} : list (VarEnv a) -> VarEnv a :=
+  UniqFM.plusUFMList.
+
+Definition plusVarEnv_C {a}
+   : (a -> a -> a) -> VarEnv a -> VarEnv a -> VarEnv a :=
+  UniqFM.plusUFM_C.
+
+Definition rnEnvL : RnEnv2 -> VarEnv Var.Var :=
+  envL.
+
+Definition rnEnvR : RnEnv2 -> VarEnv Var.Var :=
+  envR.
+
+Definition rnInScopeSet : RnEnv2 -> InScopeSet :=
+  in_scope.
+
+Definition rnSwap : RnEnv2 -> RnEnv2 :=
+  fun arg_0__ => let 'RV2 envL envR in_scope := arg_0__ in RV2 envR envL in_scope.
+
+Definition unionInScope : InScopeSet -> InScopeSet -> InScopeSet :=
+  fun arg_0__ arg_1__ =>
+    match arg_0__, arg_1__ with
+    | InScope s1 _, InScope s2 n2 => InScope (VarSet.unionVarSet s1 s2) n2
+    end.
+
+Definition uniqAway' : InScopeSet -> Var.Var -> Var.Var :=
+  fun arg_0__ arg_1__ =>
+    match arg_0__, arg_1__ with
+    | InScope set n, var =>
+        let orig_unique := Unique.getUnique var in
+        let try :=
+          GHC.DeferredFix.deferredFix1 (fun try k =>
+                                          let uniq := Unique.deriveUnique orig_unique (n GHC.Num.* k) in
+                                          let msg :=
+                                            GHC.Base.mappend (GHC.Base.mappend (GHC.Base.mappend (Panic.noString k) (id
+                                                                                                  (GHC.Base.hs_string__
+                                                                                                   "tries")))
+                                                                               (Panic.noString var)) (Panic.noString
+                                                              n) in
+                                          if andb Util.debugIsOn (k GHC.Base.> #1000) : bool
+                                          then Panic.panicStr (GHC.Base.hs_string__ "uniqAway loop:") msg else
+                                          if VarSet.elemVarSetByKey uniq set : bool then try (k GHC.Num.+ #1) else
+                                          if k GHC.Base.> #3 : bool then Var.setVarUnique var uniq else
+                                          Var.setVarUnique var uniq) in
+        try #1
+    end.
+
+Definition rnBndr2_var
+   : RnEnv2 -> Var.Var -> Var.Var -> (RnEnv2 * Var.Var)%type :=
+  fun arg_0__ arg_1__ arg_2__ =>
+    match arg_0__, arg_1__, arg_2__ with
+    | RV2 envL envR in_scope, bL, bR =>
+        let new_b :=
+          if negb (elemInScopeSet bL in_scope) : bool then bL else
+          if negb (elemInScopeSet bR in_scope) : bool then bR else
+          uniqAway' in_scope bL in
+        pair (RV2 (extendVarEnv envL bL new_b) (extendVarEnv envR bR new_b)
+                  (extendInScopeSet in_scope new_b)) new_b
+    end.
+
+Definition rnBndr2 : RnEnv2 -> Var.Var -> Var.Var -> RnEnv2 :=
+  fun env bL bR => Data.Tuple.fst (rnBndr2_var env bL bR).
+
+Definition uniqAway : InScopeSet -> Var.Var -> Var.Var :=
+  fun in_scope var =>
+    if elemInScopeSet var in_scope : bool then uniqAway' in_scope var else
+    var.
+
+Definition rnBndrL : RnEnv2 -> Var.Var -> (RnEnv2 * Var.Var)%type :=
+  fun arg_0__ arg_1__ =>
+    match arg_0__, arg_1__ with
+    | RV2 envL envR in_scope, bL =>
+        let new_b := uniqAway in_scope bL in
+        pair (RV2 (extendVarEnv envL bL new_b) envR (extendInScopeSet in_scope new_b))
+             new_b
+    end.
+
+Definition rnBndrR : RnEnv2 -> Var.Var -> (RnEnv2 * Var.Var)%type :=
+  fun arg_0__ arg_1__ =>
+    match arg_0__, arg_1__ with
+    | RV2 envL envR in_scope, bR =>
+        let new_b := uniqAway in_scope bR in
+        pair (RV2 envL (extendVarEnv envR bR new_b) (extendInScopeSet in_scope new_b))
+             new_b
+    end.
+
+Definition rnEtaL : RnEnv2 -> Var.Var -> (RnEnv2 * Var.Var)%type :=
+  fun arg_0__ arg_1__ =>
+    match arg_0__, arg_1__ with
+    | RV2 envL envR in_scope, bL =>
+        let new_b := uniqAway in_scope bL in
+        pair (RV2 (extendVarEnv envL bL new_b) (extendVarEnv envR new_b new_b)
+                  (extendInScopeSet in_scope new_b)) new_b
+    end.
+
+Definition rnEtaR : RnEnv2 -> Var.Var -> (RnEnv2 * Var.Var)%type :=
+  fun arg_0__ arg_1__ =>
+    match arg_0__, arg_1__ with
+    | RV2 envL envR in_scope, bR =>
+        let new_b := uniqAway in_scope bR in
+        pair (RV2 (extendVarEnv envL new_b new_b) (extendVarEnv envR bR new_b)
+                  (extendInScopeSet in_scope new_b)) new_b
+    end.
+
+Definition unitDVarEnv {a} : Var.Var -> a -> DVarEnv a :=
+  UniqDFM.unitUDFM.
+
+Definition unitVarEnv {a} : Var.Var -> a -> VarEnv a :=
+  UniqFM.unitUFM.
+
+Definition varSetInScope : VarSet.VarSet -> InScopeSet -> bool :=
+  fun arg_0__ arg_1__ =>
+    match arg_0__, arg_1__ with
+    | vars, InScope s1 _ => VarSet.subVarSet vars s1
+    end.
+
+(* External variables:
+     None Some andb bool list negb op_zt__ option pair Data.Foldable.foldl
+     Data.Foldable.length Data.Tuple.fst GHC.Base.mappend GHC.Base.op_zg__
+     GHC.DeferredFix.deferredFix1 GHC.Err.Default GHC.Err.default GHC.Num.Int
+     GHC.Num.fromInteger GHC.Num.op_zp__ GHC.Num.op_zt__ Maybes.orElse
+     OccName.TidyOccEnv OccName.emptyTidyOccEnv Panic.noString Panic.panicStr
+     UniqDFM.UniqDFM UniqDFM.addListToUDFM UniqDFM.addToUDFM UniqDFM.addToUDFM_C
+     UniqDFM.alterUDFM UniqDFM.anyUDFM UniqDFM.delFromUDFM UniqDFM.delListFromUDFM
+     UniqDFM.elemUDFM UniqDFM.eltsUDFM UniqDFM.emptyUDFM UniqDFM.filterUDFM
+     UniqDFM.foldUDFM UniqDFM.isNullUDFM UniqDFM.listToUDFM UniqDFM.lookupUDFM
+     UniqDFM.mapUDFM UniqDFM.minusUDFM UniqDFM.partitionUDFM UniqDFM.plusUDFM
+     UniqDFM.plusUDFM_C UniqDFM.unitUDFM UniqFM.UniqFM UniqFM.addListToUFM
+     UniqFM.addToUFM UniqFM.addToUFM_Acc UniqFM.addToUFM_C UniqFM.addToUFM_Directly
+     UniqFM.alterUFM UniqFM.delFromUFM UniqFM.delFromUFM_Directly
+     UniqFM.delListFromUFM UniqFM.disjointUFM UniqFM.elemUFM UniqFM.elemUFM_Directly
+     UniqFM.emptyUFM UniqFM.filterUFM UniqFM.filterUFM_Directly UniqFM.intersectUFM
+     UniqFM.isNullUFM UniqFM.listToUFM UniqFM.listToUFM_Directly UniqFM.lookupUFM
+     UniqFM.lookupUFM_Directly UniqFM.lookupWithDefaultUFM UniqFM.mapUFM
+     UniqFM.minusUFM UniqFM.partitionUFM UniqFM.plusMaybeUFM_C UniqFM.plusUFM
+     UniqFM.plusUFMList UniqFM.plusUFM_C UniqFM.unitUFM UniqSet.sizeUniqSet
+     Unique.Unique Unique.deriveUnique Unique.getUnique Util.debugIsOn Util.zipEqual
+     Var.Var Var.setVarUnique VarSet.VarSet VarSet.delVarSet VarSet.elemVarSet
+     VarSet.elemVarSetByKey VarSet.emptyVarSet VarSet.extendVarSet
+     VarSet.isEmptyVarSet VarSet.lookupVarSet VarSet.lookupVarSet_Directly
+     VarSet.subVarSet VarSet.unionVarSet
+*)
