examples/ghc/module-edits/IdInfo/midamble.v
@@ -1,0 +1,15 @@
+Require GHC.Err.
+
+
+Instance Default_TickBoxOp : GHC.Err.Default TickBoxOp :=
+  GHC.Err.Build_Default _ (TickBox GHC.Err.default GHC.Err.default).
+
+Instance Default_CafInfo : GHC.Err.Default CafInfo :=
+  GHC.Err.Build_Default _ MayHaveCafRefs.
+
+(*
+Instance Default_IdInfo : GHC.Err.Default IdInfo :=
+  GHC.Err.Build_Default _ (Mk_IdInfo GHC.Err.default GHC.Err.default GHC.Err.default
+                         GHC.Err.default GHC.Err.default GHC.Err.default GHC.Err.default
+                         GHC.Err.default GHC.Err.default GHC.Err.default).
+*)
