examples/ghc/module-edits/Var/midamble.v
@@ -2,17 +2,21 @@ Instance Unique_Var : Unique.Uniquable Var := {}.
 Admitted.
 
 Require Import GHC.Err.
-Instance Default__IdScope : Default IdScope := Build_Default _ GlobalId.
+
+
+(*
+Instance Default__IdScope : Default IdScope := Build_Default _ GlobalId. 
+*)
 Instance Default__Var : Default Var := Build_Default _ (Mk_Id default default default default default default).
 
 
 Instance Name_NamedThing_TyCoVar : Name.NamedThing TyCoVar.
 Admitted.
-Instance Name_NamedThing_VarId : Name.NamedThing Var.Id.
+Instance Name_NamedThing_VarId : Name.NamedThing Id.
 Admitted.
 
 
-
+(*
 Definition varType (arg_8__ : Var) :=
   match arg_8__ with
     | Core.Mk_TyVar _ _ varType => varType
@@ -34,3 +38,4 @@ Definition varName (arg_8__ : Var) :=
     | Core.Mk_TcTyVar n _ _ _ => n
     | Core.Mk_Id n _ _ _ _ _ => n
   end.
+*)
