examples/ghc/module-edits/IdInfo/preamble.v
@@ -1,0 +1,80 @@
+Require GHC.Err.
+Require GHC.Base.
+
+(* We might put these elsewhere, but these are some types that we 
+   can use for untying the knots in DataCon/Class/PatSyn *)
+
+Parameter DataConId : Type.
+Parameter ClassId   : Type.
+Parameter PatSynId  : Type.
+
+Parameter Default_DataConId : GHC.Err.Default DataConId.
+Parameter Default_ClassId   : GHC.Err.Default ClassId.
+Parameter Default_PatSynId  : GHC.Err.Default PatSynId.
+
+Parameter Eq_PatSynId  : Base.Eq_ PatSynId.
+Parameter Eq_ClassId   : Base.Eq_ ClassId.
+Parameter Eq_DataConId : Base.Eq_ DataConId.
+
+Parameter Ord_PatSynId  : Base.Ord PatSynId.
+Parameter Ord_ClassId   : Base.Ord ClassId.
+Parameter Ord_DataConId : Base.Ord DataConId.
+
+
+(*
+-- An 'IdInfo' gives /optional/ information about an 'Id'.  If
+-- present it never lies, but it may not be present, in which case there
+-- is always a conservative assumption which can be made.
+
+-- Most of the 'IdInfo' gives information about the value, or definition, of
+-- the 'Id', independent of its usage. Exceptions to this
+-- are 'demandInfo', 'occInfo', 'oneShotInfo' and 'callArityInfo'.
+--
+
+data IdInfo
+  = IdInfo {
+        arityInfo       :: !ArityInfo,          -- ^ 'Id' arity
+        ruleInfo        :: RuleInfo,            -- ^ Specialisations of the 'Id's function which exist
+                                                -- See Note [Specialisations and RULES in IdInfo]
+        unfoldingInfo   :: Unfolding,           -- ^ The 'Id's unfolding
+        cafInfo         :: CafInfo,             -- ^ 'Id' CAF info
+        oneShotInfo     :: OneShotInfo,         -- ^ Info about a lambda-bound variable, if the 'Id' is one
+        inlinePragInfo  :: InlinePragma,        -- ^ Any inline pragma atached to the 'Id'
+        occInfo         :: OccInfo,             -- ^ How the 'Id' occurs in the program
+
+        strictnessInfo  :: StrictSig,      --  ^ A strictness signature
+
+        demandInfo      :: Demand,       -- ^ ID demand information
+        callArityInfo   :: !ArityInfo,   -- ^ How this is called.
+                                         -- n <=> all calls have at least n arguments
+
+        levityInfo      :: LevityInfo    -- ^ when applied, will this Id ever have a levity-polymorphic type?
+    }
+
+*)
+
+Parameter IdInfo        : Type.
+Parameter vanillaIdInfo : IdInfo.
+Parameter noCafIdInfo   : IdInfo.
+
+Instance Default_IdInfo : GHC.Err.Default IdInfo :=
+  GHC.Err.Build_Default _ vanillaIdInfo.
+
+(* -------------------- *)
+
+Parameter RuleInfo : Type.
+Parameter emptyRuleInfo : RuleInfo.
+Parameter isEmptyRuleInfo : RuleInfo -> bool.
+
+Instance Default_RuleInfo : GHC.Err.Default RuleInfo :=
+  GHC.Err.Build_Default _ emptyRuleInfo.
+
+
+(* -------------------- *)
+
+(*
+Parameter RecSelParent : Type.
+Parameter Default_RecSelParent : GHC.Err.Default RecSelParent.
+
+Parameter Eq___RecSelParent : GHC.Base.Eq_ RecSelParent.
+*)
