examples/tests/RenameMe.hs-boot
@@ -1,0 +1,3 @@
+module RenameMe where
+
+data Odd 
